Clean Earley_Parser

Earley_Parser.thy
@@ -9,35 +9,33 @@ section \<open>Earley parser\<close>
 subsection \<open>Pointer lemmas\<close>
 
 definition predicts :: "'a item \<Rightarrow> bool" where
-  "predicts x \<longleftrightarrow> item_origin x = item_end x \<and> item_dot x = 0"
+  "predicts x \<equiv> item_origin x = item_end x \<and> item_dot x = 0"
 
 definition scans :: "'a sentence \<Rightarrow> nat \<Rightarrow> 'a item \<Rightarrow> 'a item \<Rightarrow> bool" where
-  "scans inp k x y \<longleftrightarrow> y = inc_item x k \<and> (\<exists>a. next_symbol x = Some a \<and> inp!(k-1) = a)"
+  "scans \<omega> k x y \<equiv> y = inc_item x k \<and> (\<exists>a. next_symbol x = Some a \<and> \<omega>!(k-1) = a)"
 
 definition completes :: "nat \<Rightarrow> 'a item \<Rightarrow> 'a item \<Rightarrow> 'a item \<Rightarrow> bool" where
-  "completes k x y z \<longleftrightarrow> y = inc_item x k \<and> is_complete z \<and> item_origin z = item_end x \<and>
+  "completes k x y z \<equiv> y = inc_item x k \<and> is_complete z \<and> item_origin z = item_end x \<and>
     (\<exists>N. next_symbol x = Some N \<and> N = item_rule_head z)"
 
 definition sound_null_ptr :: "'a entry \<Rightarrow> bool" where
-  "sound_null_ptr e = (pointer e = Null \<longrightarrow> predicts (item e))"
+  "sound_null_ptr e \<equiv> (pointer e = Null \<longrightarrow> predicts (item e))"
 
 definition sound_pre_ptr :: "'a sentence \<Rightarrow> 'a bins \<Rightarrow> nat \<Rightarrow> 'a entry \<Rightarrow> bool" where
-  "sound_pre_ptr inp bs k e = (\<forall>pre. pointer e = Pre pre \<longrightarrow>
-    k > 0 \<and> pre < length (bs!(k-1)) \<and> scans inp k (item (bs!(k-1)!pre)) (item e))"
+  "sound_pre_ptr \<omega> bs k e \<equiv> \<forall>pre. pointer e = Pre pre \<longrightarrow>
+    k > 0 \<and> pre < length (bs!(k-1)) \<and> scans \<omega> k (item (bs!(k-1)!pre)) (item e)"
 
 definition sound_prered_ptr :: "'a bins \<Rightarrow> nat \<Rightarrow> 'a entry \<Rightarrow> bool" where
-  "sound_prered_ptr bs k e = (\<forall>p ps k' pre red. pointer e = PreRed p ps \<and> (k', pre, red) \<in> set (p#ps) \<longrightarrow>
-    k' < k \<and> pre < length (bs!k') \<and> red < length (bs!k) \<and> completes k (item (bs!k'!pre)) (item e) (item (bs!k!red)))"
+  "sound_prered_ptr bs k e \<equiv> \<forall>p ps k' pre red. pointer e = PreRed p ps \<and> (k', pre, red) \<in> set (p#ps) \<longrightarrow>
+    k' < k \<and> pre < length (bs!k') \<and> red < length (bs!k) \<and> completes k (item (bs!k'!pre)) (item e) (item (bs!k!red))"
 
 definition sound_ptrs :: "'a sentence \<Rightarrow> 'a bins \<Rightarrow> bool" where
-  "sound_ptrs inp bs = (\<forall>k < length bs. \<forall>e \<in> set (bs!k).
-    sound_null_ptr e \<and>
-    sound_pre_ptr inp bs k e \<and>
-    sound_prered_ptr bs k e)"
+  "sound_ptrs \<omega> bs \<equiv> \<forall>k < length bs. \<forall>e \<in> set (bs!k).
+    sound_null_ptr e \<and> sound_pre_ptr \<omega> bs k e \<and> sound_prered_ptr bs k e"
 
 definition mono_red_ptr :: "'a bins \<Rightarrow> bool" where
-  "mono_red_ptr bs = (\<forall>k < length bs. \<forall>i < length (bs!k).
-    \<forall>k' pre red ps. pointer (bs!k!i) = PreRed (k', pre, red) ps \<longrightarrow> red < i)"
+  "mono_red_ptr bs \<equiv> \<forall>k < length bs. \<forall>i < length (bs!k).
+    \<forall>k' pre red ps. pointer (bs!k!i) = PreRed (k', pre, red) ps \<longrightarrow> red < i"
 
 lemma nth_item_bin_upd:
   "n < length es \<Longrightarrow> item (bin_upd e es ! n) = item (es!n)"
@@ -113,25 +111,25 @@ proof (induction es arbitrary: e i es')
 qed simp
 
 lemma sound_ptrs_bin_upd:
-  assumes "sound_ptrs inp bs" "k < length bs" "es = bs!k" "distinct (items es)"
-  assumes "sound_null_ptr e" "sound_pre_ptr inp bs k e" "sound_prered_ptr bs k e"
-  shows "sound_ptrs inp (bs[k := bin_upd e es])"
+  assumes "sound_ptrs \<omega> bs" "k < length bs" "es = bs!k" "distinct (items es)"
+  assumes "sound_null_ptr e" "sound_pre_ptr \<omega> bs k e" "sound_prered_ptr bs k e"
+  shows "sound_ptrs \<omega> (bs[k := bin_upd e es])"
   unfolding sound_ptrs_def
 proof (standard, standard, standard)
   fix idx elem
   let ?bs = "bs[k := bin_upd e es]"
   assume a0: "idx < length ?bs"
   assume a1: "elem \<in> set (?bs ! idx)"
-  show "sound_null_ptr elem \<and> sound_pre_ptr inp ?bs idx elem \<and> sound_prered_ptr ?bs idx elem"
+  show "sound_null_ptr elem \<and> sound_pre_ptr \<omega> ?bs idx elem \<and> sound_prered_ptr ?bs idx elem"
   proof cases
     assume a2: "idx = k"
-    have "elem \<in> set es \<Longrightarrow> sound_pre_ptr inp bs idx elem"
+    have "elem \<in> set es \<Longrightarrow> sound_pre_ptr \<omega> bs idx elem"
       using a0 a2 assms(1-3) sound_ptrs_def by blast
-    hence pre_es: "elem \<in> set es \<Longrightarrow> sound_pre_ptr inp ?bs idx elem"
+    hence pre_es: "elem \<in> set es \<Longrightarrow> sound_pre_ptr \<omega> ?bs idx elem"
       using a2 unfolding sound_pre_ptr_def by force
-    have "elem = e \<Longrightarrow> sound_pre_ptr inp bs idx elem"
+    have "elem = e \<Longrightarrow> sound_pre_ptr \<omega> bs idx elem"
       using a2 assms(6) by auto
-    hence pre_e: "elem = e \<Longrightarrow> sound_pre_ptr inp ?bs idx elem"
+    hence pre_e: "elem = e \<Longrightarrow> sound_pre_ptr \<omega> ?bs idx elem"
       using a2 unfolding sound_pre_ptr_def by force
     have "elem \<in> set es \<Longrightarrow> sound_prered_ptr bs idx elem"
       using a0 a2 assms(1-3) sound_ptrs_def by blast
@@ -186,7 +184,7 @@ proof (standard, standard, standard)
             using 0 1 by blast
           have "sound_null_ptr elem"
             using a3 unfolding sound_null_ptr_def by simp
-          moreover have "sound_pre_ptr inp ?bs idx elem"
+          moreover have "sound_pre_ptr \<omega> ?bs idx elem"
             using a3 unfolding sound_pre_ptr_def by simp
           moreover have "sound_prered_ptr ?bs idx elem"
             unfolding sound_prered_ptr_def
@@ -227,9 +225,9 @@ proof (standard, standard, standard)
     assume a2: "idx \<noteq> k"
     have null: "sound_null_ptr elem"
       using a0 a1 a2 assms(1) sound_ptrs_def by auto
-    have "sound_pre_ptr inp bs idx elem"
+    have "sound_pre_ptr \<omega> bs idx elem"
       using a0 a1 a2 assms(1,2) unfolding sound_ptrs_def by simp
-    hence pre: "sound_pre_ptr inp ?bs idx elem"
+    hence pre: "sound_pre_ptr \<omega> ?bs idx elem"
       using assms(2,3) length_bin_upd nth_item_bin_upd unfolding sound_pre_ptr_def
       using dual_order.strict_trans1 nth_list_update by fastforce
     have "sound_prered_ptr bs idx elem"
@@ -319,15 +317,15 @@ proof (standard, standard)
 qed
 
 lemma sound_mono_ptrs_bin_upds:
-  assumes "sound_ptrs inp bs" "mono_red_ptr bs" "k < length bs" "b = bs!k" "distinct (items b)" "distinct (items es)"
-  assumes "\<forall>e \<in> set es. sound_null_ptr e \<and> sound_pre_ptr inp bs k e \<and> sound_prered_ptr bs k e"
+  assumes "sound_ptrs \<omega> bs" "mono_red_ptr bs" "k < length bs" "b = bs!k" "distinct (items b)" "distinct (items es)"
+  assumes "\<forall>e \<in> set es. sound_null_ptr e \<and> sound_pre_ptr \<omega> bs k e \<and> sound_prered_ptr bs k e"
   assumes "\<forall>e \<in> set es. \<forall>k' pre red ps. pointer e = PreRed (k', pre, red) ps \<longrightarrow> red < length b"
-  shows "sound_ptrs inp (bs[k := bin_upds es b]) \<and> mono_red_ptr (bs[k := bin_upds es b])"
+  shows "sound_ptrs \<omega> (bs[k := bin_upds es b]) \<and> mono_red_ptr (bs[k := bin_upds es b])"
   using assms
 proof (induction es arbitrary: b bs)
   case (Cons e es)
   let ?bs = "bs[k := bin_upd e b]"
-  have 0: "sound_ptrs inp ?bs"
+  have 0: "sound_ptrs \<omega> ?bs"
     using sound_ptrs_bin_upd Cons.prems(1,3-5,7) by (metis list.set_intros(1))
   have 1: "mono_red_ptr ?bs"
     using mono_red_ptr_bin_upd Cons.prems(2-5,8) by auto
@@ -335,12 +333,12 @@ proof (induction es arbitrary: b bs)
     using Cons.prems(3) by simp
   have 3: "bin_upd e b = ?bs!k"
     using Cons.prems(3) by simp
-  have 4: "\<forall>e' \<in> set es. sound_null_ptr e' \<and> sound_pre_ptr inp ?bs k e' \<and> sound_prered_ptr ?bs k e'"
+  have 4: "\<forall>e' \<in> set es. sound_null_ptr e' \<and> sound_pre_ptr \<omega> ?bs k e' \<and> sound_prered_ptr ?bs k e'"
     using Cons.prems(3,4,7) length_bin_upd nth_item_bin_upd sound_pre_ptr_def sound_prered_ptr_def
     by (smt (verit, ccfv_threshold) list.set_intros(2) nth_list_update order_less_le_trans)
   have 5: "\<forall>e' \<in> set es. \<forall>k' pre red ps. pointer e' = PreRed (k', pre, red) ps \<longrightarrow> red < length (bin_upd e b)"
     by (meson Cons.prems(8) length_bin_upd order_less_le_trans set_subset_Cons subsetD)
-  have "sound_ptrs inp ((bs[k := bin_upd e b])[k := bin_upds es (bin_upd e b)]) \<and>
+  have "sound_ptrs \<omega> ((bs[k := bin_upd e b])[k := bin_upds es (bin_upd e b)]) \<and>
     mono_red_ptr (bs[k := bin_upd e b, k := bin_upds es (bin_upd e b)])"
     using Cons.IH[OF 0 1 2 3 _ _ 4 5] distinct_bin_upd Cons.prems(4,5,6) items_def by (metis distinct.simps(2) list.simps(9))
   thus ?case
@@ -348,27 +346,27 @@ proof (induction es arbitrary: b bs)
 qed simp
 
 lemma sound_mono_ptrs_Earley\<^sub>L_bin':
-  assumes "(k, cfg, inp, bs) \<in> wf_earley_input"
-  assumes "sound_ptrs inp bs" "\<forall>x \<in> bins bs. sound_item cfg inp x"
+  assumes "(k, \<G>, \<omega>, bs) \<in> wf_earley_input"
+  assumes "sound_ptrs \<omega> bs" "\<forall>x \<in> bins bs. sound_item \<G> \<omega> x"
   assumes "mono_red_ptr bs"
-  assumes "nonempty_derives cfg" "wf_\<G> cfg"
-  shows "sound_ptrs inp (Earley\<^sub>L_bin' k cfg inp bs i) \<and> mono_red_ptr (Earley\<^sub>L_bin' k cfg inp bs i)"
+  assumes "nonempty_derives \<G>" "wf_\<G> \<G>"
+  shows "sound_ptrs \<omega> (Earley\<^sub>L_bin' k \<G> \<omega> bs i) \<and> mono_red_ptr (Earley\<^sub>L_bin' k \<G> \<omega> bs i)"
   using assms
 proof (induction i rule: Earley\<^sub>L_bin'_induct[OF assms(1), case_names Base Complete\<^sub>F Scan\<^sub>F Pass Predict\<^sub>F])
-  case (Complete\<^sub>F k cfg inp bs i x)
+  case (Complete\<^sub>F k \<G> \<omega> bs i x)
   let ?bs' = "bins_upd bs k (Complete\<^sub>L k x bs i)"
   have x: "x \<in> set (items (bs ! k))"
     using Complete\<^sub>F.hyps(1,2) by force
-  hence "\<forall>x \<in> set (items (Complete\<^sub>L k x bs i)). sound_item cfg inp x"
+  hence "\<forall>x \<in> set (items (Complete\<^sub>L k x bs i)). sound_item \<G> \<omega> x"
     using sound_Complete\<^sub>L Complete\<^sub>F.hyps(3) Complete\<^sub>F.prems wf_earley_input_elim wf_bins_impl_wf_items x
     by (metis dual_order.refl)
-  hence sound: "\<forall>x \<in> bins ?bs'. sound_item cfg inp x"
+  hence sound: "\<forall>x \<in> bins ?bs'. sound_item \<G> \<omega> x"
     by (metis Complete\<^sub>F.prems(1,3) UnE bins_bins_upd wf_earley_input_elim)
   have 0: "k < length bs"
     using Complete\<^sub>F.prems(1) wf_earley_input_elim by auto
   have 1: "\<forall>e \<in> set (Complete\<^sub>L k x bs i). sound_null_ptr e"
     unfolding Complete\<^sub>L_def sound_null_ptr_def by auto
-  have 2: "\<forall>e \<in> set (Complete\<^sub>L k x bs i). sound_pre_ptr inp bs k e"
+  have 2: "\<forall>e \<in> set (Complete\<^sub>L k x bs i). sound_pre_ptr \<omega> bs k e"
     unfolding Complete\<^sub>L_def sound_pre_ptr_def by auto
   {
     fix e
@@ -377,33 +375,42 @@ proof (induction i rule: Earley\<^sub>L_bin'_induct[OF assms(1), case_names Base
     assume a1: "pointer e = PreRed p ps" "(k', pre, red) \<in> set (p#ps)"
     have "k' = item_origin x"
       using a0 a1 unfolding Complete\<^sub>L_def by auto
-    moreover have "wf_item cfg inp x" "item_end x = k"
+    moreover have "wf_item \<G> \<omega> x" "item_end x = k"
       using Complete\<^sub>F.prems(1) x wf_earley_input_elim wf_bins_kth_bin by blast+
     ultimately have 0: "k' \<le> k"
       using wf_item_def by blast
     have 1: "k' \<noteq> k"
     proof (rule ccontr)
       assume "\<not> k' \<noteq> k"
-      have "sound_item cfg inp x"
+      have "sound_item \<G> \<omega> x"
         using Complete\<^sub>F.prems(1,3) x kth_bin_sub_bins wf_earley_input_elim by (metis subset_eq)
       moreover have "is_complete x"
         using Complete\<^sub>F.hyps(3) by (auto simp: next_symbol_def split: if_splits)
       moreover have "item_origin x = k"
         using \<open>\<not> k' \<noteq> k\<close> \<open>k' = item_origin x\<close> by auto
       ultimately show False
-        using impossible_complete_item Complete\<^sub>F.prems(1,5) wf_earley_input_elim \<open>item_end x = k\<close> \<open>wf_item cfg inp x\<close> by blast
+        using impossible_complete_item Complete\<^sub>F.prems(1,5) wf_earley_input_elim \<open>item_end x = k\<close> \<open>wf_item \<G> \<omega> x\<close> by blast
     qed
     have 2: "pre < length (bs!k')"
       using a0 a1 index_filter_with_index_lt_length unfolding Complete\<^sub>L_def by (auto simp: items_def; fastforce)
     have 3: "red < i+1"
       using a0 a1 unfolding Complete\<^sub>L_def by auto
-    have 4: "completes k (item (bs!k'!pre)) (item e) (item (bs!k!red))"
-      using a0 a1 0 2 Complete\<^sub>F.hyps(1,2,3) Complete\<^sub>F.prems(1) \<open>k' = item_origin x\<close> unfolding Complete\<^sub>L_def completes_def
+
+    have "item e = inc_item (item (bs!k'!pre)) k"
+      using a0 a1 0 2 Complete\<^sub>F.hyps(1,2,3) Complete\<^sub>F.prems(1) \<open>k' = item_origin x\<close> unfolding Complete\<^sub>L_def
+      by (auto simp: items_def, metis filter_with_index_nth nth_map)
+    moreover have "is_complete (item (bs!k!red))"
+      using a0 a1 0 2 Complete\<^sub>F.hyps(1,2,3) Complete\<^sub>F.prems(1) \<open>k' = item_origin x\<close> unfolding Complete\<^sub>L_def
+      by (auto simp: next_symbol_def items_def split: if_splits)
+    moreover have "item_origin (item (bs!k!red)) = item_end (item (bs!k'!pre))"
+      using a0 a1 0 2 Complete\<^sub>F.hyps(1,2,3) Complete\<^sub>F.prems(1) \<open>k' = item_origin x\<close> unfolding Complete\<^sub>L_def
       apply (auto simp: items_def)
-      apply (metis filter_with_index_nth nth_map)
-      apply (metis next_symbol_def option.discI)
-      apply (metis items_def index_filter_with_index_lt_length nth_map nth_mem order_le_less_trans wf_earley_input_elim wf_bins_kth_bin)
-      by (metis (mono_tags, lifting) filter_with_index_P filter_with_index_nth items_def linorder_not_less nth_map)
+      by (metis dual_order.strict_trans index_filter_with_index_lt_length items_def le_neq_implies_less nth_map nth_mem wf_bins_kth_bin wf_earley_input_elim)
+    moreover have "(\<exists>N. next_symbol (item (bs ! k' ! pre)) = Some N \<and> N = item_rule_head (item (bs ! k ! red)))"
+      using a0 a1 0 2 Complete\<^sub>F.hyps(1,2,3) Complete\<^sub>F.prems(1) \<open>k' = item_origin x\<close> unfolding Complete\<^sub>L_def
+      by (auto simp: items_def, metis (mono_tags, lifting) filter_with_index_P filter_with_index_nth nth_map)
+    ultimately have 4: "completes k (item (bs!k'!pre)) (item e) (item (bs!k!red))"
+      unfolding completes_def by blast
     have "k' < k" "pre < length (bs!k')" "red < i+1" "completes k (item (bs!k'!pre)) (item e) (item (bs!k!red))"
       using 0 1 2 3 4 by simp_all
   }
@@ -415,123 +422,124 @@ proof (induction i rule: Earley\<^sub>L_bin'_induct[OF assms(1), case_names Base
   have 4: "distinct (items (Complete\<^sub>L k x bs i))"
     using distinct_Complete\<^sub>L x Complete\<^sub>F.prems(1) wf_earley_input_elim wf_bin_def wf_bin_items_def wf_bins_def wf_item_def
     by (metis order_le_less_trans)
-  have "sound_ptrs inp ?bs' \<and> mono_red_ptr ?bs'"
+  have "sound_ptrs \<omega> ?bs' \<and> mono_red_ptr ?bs'"
     using sound_mono_ptrs_bin_upds[OF Complete\<^sub>F.prems(2) Complete\<^sub>F.prems(4) 0] 1 2 3 4 sound_prered_ptr_def
       Complete\<^sub>F.prems(1) bins_upd_def wf_earley_input_elim wf_bin_def wf_bins_def
     by (smt (verit, ccfv_SIG) list.set_intros(1))
-  moreover have "(k, cfg, inp, ?bs') \<in> wf_earley_input"
+  moreover have "(k, \<G>, \<omega>, ?bs') \<in> wf_earley_input"
     using Complete\<^sub>F.hyps Complete\<^sub>F.prems(1) wf_earley_input_Complete\<^sub>L by blast
-  ultimately have "sound_ptrs inp (Earley\<^sub>L_bin' k cfg inp ?bs' (i+1)) \<and> mono_red_ptr (Earley\<^sub>L_bin' k cfg inp ?bs' (i+1))"
+  ultimately have "sound_ptrs \<omega> (Earley\<^sub>L_bin' k \<G> \<omega> ?bs' (i+1)) \<and> mono_red_ptr (Earley\<^sub>L_bin' k \<G> \<omega> ?bs' (i+1))"
     using Complete\<^sub>F.IH Complete\<^sub>F.prems(4-6) sound by blast
   thus ?case
     using Complete\<^sub>F.hyps by simp
 next
-  case (Scan\<^sub>F k cfg inp bs i x a)
-  let ?bs' = "bins_upd bs (k+1) (Scan\<^sub>L k inp a x i)"
+  case (Scan\<^sub>F k \<G> \<omega> bs i x a)
+  let ?bs' = "bins_upd bs (k+1) (Scan\<^sub>L k \<omega> a x i)"
   have "x \<in> set (items (bs ! k))"
     using Scan\<^sub>F.hyps(1,2) by force
-  hence "\<forall>x \<in> set (items (Scan\<^sub>L k inp a x i)). sound_item cfg inp x"
+  hence "\<forall>x \<in> set (items (Scan\<^sub>L k \<omega> a x i)). sound_item \<G> \<omega> x"
     using sound_Scan\<^sub>L Scan\<^sub>F.hyps(3,5) Scan\<^sub>F.prems(1,2,3) wf_earley_input_elim wf_bins_impl_wf_items wf_bins_impl_wf_items by fast
-  hence sound: "\<forall>x \<in> bins ?bs'. sound_item cfg inp x"
+  hence sound: "\<forall>x \<in> bins ?bs'. sound_item \<G> \<omega> x"
     using Scan\<^sub>F.hyps(5) Scan\<^sub>F.prems(1,3) bins_bins_upd wf_earley_input_elim
     by (metis UnE add_less_cancel_right)
   have 0: "k+1 < length bs"
     using Scan\<^sub>F.hyps(5) Scan\<^sub>F.prems(1) wf_earley_input_elim by force
-  have 1: "\<forall>e \<in> set (Scan\<^sub>L k inp a x i). sound_null_ptr e"
+  have 1: "\<forall>e \<in> set (Scan\<^sub>L k \<omega> a x i). sound_null_ptr e"
     unfolding Scan\<^sub>L_def sound_null_ptr_def by auto
-  have 2: "\<forall>e \<in> set (Scan\<^sub>L k inp a x i). sound_pre_ptr inp bs (k+1) e"
+  have 2: "\<forall>e \<in> set (Scan\<^sub>L k \<omega> a x i). sound_pre_ptr \<omega> bs (k+1) e"
     using Scan\<^sub>F.hyps(1,2,3) unfolding sound_pre_ptr_def Scan\<^sub>L_def scans_def items_def by auto
-  have 3: "\<forall>e \<in> set (Scan\<^sub>L k inp a x i). sound_prered_ptr bs (k+1) e"
+  have 3: "\<forall>e \<in> set (Scan\<^sub>L k \<omega> a x i). sound_prered_ptr bs (k+1) e"
     unfolding Scan\<^sub>L_def sound_prered_ptr_def by simp
-  have 4: "distinct (items (Scan\<^sub>L k inp a x i))"
+  have 4: "distinct (items (Scan\<^sub>L k \<omega> a x i))"
     using distinct_Scan\<^sub>L by fast
-  have "sound_ptrs inp ?bs' \<and> mono_red_ptr ?bs'"
+  have "sound_ptrs \<omega> ?bs' \<and> mono_red_ptr ?bs'"
     using sound_mono_ptrs_bin_upds[OF Scan\<^sub>F.prems(2) Scan\<^sub>F.prems(4) 0] 0 1 2 3 4 sound_prered_ptr_def
       Scan\<^sub>F.prems(1) bins_upd_def wf_earley_input_elim wf_bin_def wf_bins_def
     by (smt (verit, ccfv_threshold) list.set_intros(1))
-  moreover have "(k, cfg, inp, ?bs') \<in> wf_earley_input"
+  moreover have "(k, \<G>, \<omega>, ?bs') \<in> wf_earley_input"
     using Scan\<^sub>F.hyps Scan\<^sub>F.prems(1) wf_earley_input_Scan\<^sub>L by metis
-  ultimately have "sound_ptrs inp (Earley\<^sub>L_bin' k cfg inp ?bs' (i+1)) \<and> mono_red_ptr (Earley\<^sub>L_bin' k cfg inp ?bs' (i+1))"
+  ultimately have "sound_ptrs \<omega> (Earley\<^sub>L_bin' k \<G> \<omega> ?bs' (i+1)) \<and> mono_red_ptr (Earley\<^sub>L_bin' k \<G> \<omega> ?bs' (i+1))"
     using Scan\<^sub>F.IH Scan\<^sub>F.prems(4-6) sound by blast
   thus ?case
     using Scan\<^sub>F.hyps by simp
 next
-  case (Predict\<^sub>F k cfg inp bs i x a)
-  let ?bs' = "bins_upd bs k (Predict\<^sub>L k cfg a)"
+  case (Predict\<^sub>F k \<G> \<omega> bs i x a)
+  let ?bs' = "bins_upd bs k (Predict\<^sub>L k \<G> a)"
   have "x \<in> set (items (bs ! k))"
     using Predict\<^sub>F.hyps(1,2) by force
-  hence "\<forall>x \<in> set (items(Predict\<^sub>L k cfg a)). sound_item cfg inp x"
+  hence "\<forall>x \<in> set (items(Predict\<^sub>L k \<G> a)). sound_item \<G> \<omega> x"
     using sound_Predict\<^sub>L Predict\<^sub>F.hyps(3) Predict\<^sub>F.prems wf_earley_input_elim wf_bins_impl_wf_items by fast
-  hence sound: "\<forall>x \<in> bins ?bs'. sound_item cfg inp x"
+  hence sound: "\<forall>x \<in> bins ?bs'. sound_item \<G> \<omega> x"
     using Predict\<^sub>F.prems(1,3) UnE bins_bins_upd wf_earley_input_elim by metis
   have 0: "k < length bs"
     using Predict\<^sub>F.prems(1) wf_earley_input_elim by force
-  have 1: "\<forall>e \<in> set (Predict\<^sub>L k cfg a). sound_null_ptr e"
+  have 1: "\<forall>e \<in> set (Predict\<^sub>L k \<G> a). sound_null_ptr e"
     unfolding sound_null_ptr_def Predict\<^sub>L_def predicts_def by (auto simp: init_item_def)
-  have 2: "\<forall>e \<in> set (Predict\<^sub>L k cfg a). sound_pre_ptr inp bs k e"
+  have 2: "\<forall>e \<in> set (Predict\<^sub>L k \<G> a). sound_pre_ptr \<omega> bs k e"
     unfolding sound_pre_ptr_def Predict\<^sub>L_def by simp
-  have 3: "\<forall>e \<in> set (Predict\<^sub>L k cfg a). sound_prered_ptr bs k e"
+  have 3: "\<forall>e \<in> set (Predict\<^sub>L k \<G> a). sound_prered_ptr bs k e"
     unfolding sound_prered_ptr_def Predict\<^sub>L_def by simp
-  have 4: "distinct (items (Predict\<^sub>L k cfg a))"
+  have 4: "distinct (items (Predict\<^sub>L k \<G> a))"
     using Predict\<^sub>F.prems(6) distinct_Predict\<^sub>L by fast
-  have "sound_ptrs inp ?bs' \<and> mono_red_ptr ?bs'"
+  have "sound_ptrs \<omega> ?bs' \<and> mono_red_ptr ?bs'"
     using sound_mono_ptrs_bin_upds[OF Predict\<^sub>F.prems(2) Predict\<^sub>F.prems(4) 0] 0 1 2 3 4 sound_prered_ptr_def
       Predict\<^sub>F.prems(1) bins_upd_def wf_earley_input_elim wf_bin_def wf_bins_def
     by (smt (verit, ccfv_threshold) list.set_intros(1))
-  moreover have "(k, cfg, inp, ?bs') \<in> wf_earley_input"
+  moreover have "(k, \<G>, \<omega>, ?bs') \<in> wf_earley_input"
     using Predict\<^sub>F.hyps Predict\<^sub>F.prems(1) wf_earley_input_Predict\<^sub>L by metis
-  ultimately have "sound_ptrs inp (Earley\<^sub>L_bin' k cfg inp ?bs' (i+1)) \<and> mono_red_ptr (Earley\<^sub>L_bin' k cfg inp ?bs' (i+1))"
+  ultimately have "sound_ptrs \<omega> (Earley\<^sub>L_bin' k \<G> \<omega> ?bs' (i+1)) \<and> mono_red_ptr (Earley\<^sub>L_bin' k \<G> \<omega> ?bs' (i+1))"
     using Predict\<^sub>F.IH Predict\<^sub>F.prems(4-6) sound by blast
   thus ?case
     using Predict\<^sub>F.hyps by simp
 qed simp_all
 
 lemma sound_mono_ptrs_Earley\<^sub>L_bin:
-  assumes "(k, cfg, inp, bs) \<in> wf_earley_input"
-  assumes "sound_ptrs inp bs" "\<forall>x \<in> bins bs. sound_item cfg inp x"
+  assumes "(k, \<G>, \<omega>, bs) \<in> wf_earley_input"
+  assumes "sound_ptrs \<omega> bs" "\<forall>x \<in> bins bs. sound_item \<G> \<omega> x"
   assumes "mono_red_ptr bs"
-  assumes "nonempty_derives cfg" "wf_\<G> cfg"
-  shows "sound_ptrs inp (Earley\<^sub>L_bin k cfg inp bs) \<and> mono_red_ptr (Earley\<^sub>L_bin k cfg inp bs)"
+  assumes "nonempty_derives \<G>" "wf_\<G> \<G>"
+  shows "sound_ptrs \<omega> (Earley\<^sub>L_bin k \<G> \<omega> bs) \<and> mono_red_ptr (Earley\<^sub>L_bin k \<G> \<omega> bs)"
   using assms sound_mono_ptrs_Earley\<^sub>L_bin' Earley\<^sub>L_bin_def by metis
 
 lemma sound_ptrs_Init\<^sub>L:
-  "sound_ptrs inp (Init\<^sub>L cfg inp)"
+  "sound_ptrs \<omega> (Init\<^sub>L \<G> \<omega>)"
   unfolding sound_ptrs_def sound_null_ptr_def sound_pre_ptr_def sound_prered_ptr_def
     predicts_def scans_def completes_def Init\<^sub>L_def
   by (auto simp: init_item_def less_Suc_eq_0_disj)
 
 lemma mono_red_ptr_Init\<^sub>L:
-  "mono_red_ptr (Init\<^sub>L cfg inp)"
+  "mono_red_ptr (Init\<^sub>L \<G> \<omega>)"
   unfolding mono_red_ptr_def Init\<^sub>L_def
   by (auto simp: init_item_def less_Suc_eq_0_disj)
 
 lemma sound_mono_ptrs_Earley\<^sub>L_bins:
-  assumes "k \<le> length inp" "wf_\<G> cfg" "nonempty_derives cfg" "wf_\<G> cfg"
-  shows "sound_ptrs inp (Earley\<^sub>L_bins k cfg inp) \<and> mono_red_ptr (Earley\<^sub>L_bins k cfg inp)"
+  assumes "k \<le> length \<omega>" "wf_\<G> \<G>" "nonempty_derives \<G>" "wf_\<G> \<G>"
+  shows "sound_ptrs \<omega> (Earley\<^sub>L_bins k \<G> \<omega>) \<and> mono_red_ptr (Earley\<^sub>L_bins k \<G> \<omega>)"
   using assms
 proof (induction k)
   case 0
-  have "(0, cfg, inp, (Init\<^sub>L cfg inp)) \<in> wf_earley_input"
+  have "(0, \<G>, \<omega>, (Init\<^sub>L \<G> \<omega>)) \<in> wf_earley_input"
     using assms(2) wf_earley_input_Init\<^sub>L by blast
-  moreover have "\<forall>x \<in> bins (Init\<^sub>L cfg inp). sound_item cfg inp x"
+  moreover have "\<forall>x \<in> bins (Init\<^sub>L \<G> \<omega>). sound_item \<G> \<omega> x"
     by (metis Init\<^sub>L_eq_Init\<^sub>F Init\<^sub>F_sub_Earley sound_Earley subsetD wf_Earley)
   ultimately show ?case
     using sound_mono_ptrs_Earley\<^sub>L_bin sound_ptrs_Init\<^sub>L mono_red_ptr_Init\<^sub>L "0.prems"(2,3) by fastforce
 next
   case (Suc k)
-  have "(Suc k, cfg, inp, Earley\<^sub>L_bins k cfg inp) \<in> wf_earley_input"
+  have "(Suc k, \<G>, \<omega>, Earley\<^sub>L_bins k \<G> \<omega>) \<in> wf_earley_input"
     by (simp add: Suc.prems(1) Suc_leD assms(2) wf_earley_input_intro)
-  moreover have "sound_ptrs inp (Earley\<^sub>L_bins k cfg inp)"
+  moreover have "sound_ptrs \<omega> (Earley\<^sub>L_bins k \<G> \<omega>)"
     using Suc by simp
-  moreover have "\<forall>x \<in> bins (Earley\<^sub>L_bins k cfg inp). sound_item cfg inp x"
-    by (meson Suc.prems(1) Suc_leD Earley\<^sub>L_bins_sub_Earley\<^sub>F_bins Earley\<^sub>F_bins_sub_Earley assms(2) sound_Earley subsetD wf_bins_Earley\<^sub>L_bins wf_bins_impl_wf_items)
+  moreover have "\<forall>x \<in> bins (Earley\<^sub>L_bins k \<G> \<omega>). sound_item \<G> \<omega> x"
+    by (meson Suc.prems(1) Suc_leD Earley\<^sub>L_bins_sub_Earley\<^sub>F_bins Earley\<^sub>F_bins_sub_Earley assms(2)
+        sound_Earley subsetD wf_bins_Earley\<^sub>L_bins wf_bins_impl_wf_items)
   ultimately show ?case
     using Suc.prems(1,3,4) sound_mono_ptrs_Earley\<^sub>L_bin Suc.IH by fastforce
 qed
 
 lemma sound_mono_ptrs_Earley\<^sub>L:
-  assumes "wf_\<G> cfg" "nonempty_derives cfg"
-  shows "sound_ptrs inp (Earley\<^sub>L cfg inp) \<and> mono_red_ptr (Earley\<^sub>L cfg inp)"
+  assumes "wf_\<G> \<G>" "nonempty_derives \<G>"
+  shows "sound_ptrs \<omega> (Earley\<^sub>L \<G> \<omega>) \<and> mono_red_ptr (Earley\<^sub>L \<G> \<omega>)"
   using assms sound_mono_ptrs_Earley\<^sub>L_bins Earley\<^sub>L_def by (metis dual_order.refl)
 
 
@@ -551,18 +559,18 @@ fun root_tree :: "'a tree \<Rightarrow> 'a" where
 
 fun wf_rule_tree :: "'a cfg \<Rightarrow> 'a tree \<Rightarrow> bool" where
   "wf_rule_tree _ (Leaf a) \<longleftrightarrow> True"
-| "wf_rule_tree cfg (Branch N ts) \<longleftrightarrow> (
-    (\<exists>r \<in> set (\<RR> cfg). N = rule_head r \<and> map root_tree ts = rule_body r) \<and>
-    (\<forall>t \<in> set ts. wf_rule_tree cfg t))"
+| "wf_rule_tree \<G> (Branch N ts) \<longleftrightarrow> (
+    (\<exists>r \<in> set (\<RR> \<G>). N = rule_head r \<and> map root_tree ts = rule_body r) \<and>
+    (\<forall>t \<in> set ts. wf_rule_tree \<G> t))"
 
 fun wf_item_tree :: "'a cfg \<Rightarrow> 'a item \<Rightarrow> 'a tree \<Rightarrow> bool" where
-  "wf_item_tree cfg _ (Leaf a) \<longleftrightarrow> True"
-| "wf_item_tree cfg x (Branch N ts) \<longleftrightarrow> (
+  "wf_item_tree \<G> _ (Leaf a) \<longleftrightarrow> True"
+| "wf_item_tree \<G> x (Branch N ts) \<longleftrightarrow> (
     N = item_rule_head x \<and> map root_tree ts = take (item_dot x) (item_rule_body x) \<and>
-    (\<forall>t \<in> set ts. wf_rule_tree cfg t))"
+    (\<forall>t \<in> set ts. wf_rule_tree \<G> t))"
 
 definition wf_yield_tree :: "'a sentence \<Rightarrow> 'a item \<Rightarrow> 'a tree \<Rightarrow> bool" where
-  "wf_yield_tree inp x t \<longleftrightarrow> yield_tree t = slice (item_origin x) (item_end x) inp"
+  "wf_yield_tree \<omega> x t \<longleftrightarrow> yield_tree t = slice (item_origin x) (item_end x) \<omega>"
 
 datatype 'a forest =
   FLeaf 'a
@@ -616,7 +624,7 @@ lemma trees_append_single_singleton:
   by (subst trees_append_singleton, auto)
 
 
-subsection \<open>Random foldl lemmas\<close>
+subsection \<open>foldl lemmas\<close>
 
 lemma foldl_add_nth:
   "k < length xs \<Longrightarrow> foldl (+) z (map length (take k xs)) + length (xs!k) = foldl (+) z (map length (take (k+1) xs))"
@@ -719,24 +727,24 @@ qed simp
 subsection \<open>Parse tree\<close>
 
 partial_function (option) build_tree' :: "'a bins \<Rightarrow> 'a sentence \<Rightarrow> nat \<Rightarrow> nat \<Rightarrow> 'a tree option" where
-  "build_tree' bs inp k i = (
+  "build_tree' bs \<omega> k i = (
     let e = bs!k!i in (
     case pointer e of
       Null \<Rightarrow> Some (Branch (item_rule_head (item e)) []) \<comment>\<open>start building sub-tree\<close>
     | Pre pre \<Rightarrow> ( \<comment>\<open>add sub-tree starting from terminal\<close>
         do {
-          t \<leftarrow> build_tree' bs inp (k-1) pre;
+          t \<leftarrow> build_tree' bs \<omega> (k-1) pre;
           case t of
-            Branch N ts \<Rightarrow> Some (Branch N (ts @ [Leaf (inp!(k-1))]))
+            Branch N ts \<Rightarrow> Some (Branch N (ts @ [Leaf (\<omega>!(k-1))]))
           | _ \<Rightarrow> undefined \<comment>\<open>impossible case\<close>
         })
     | PreRed (k', pre, red) _ \<Rightarrow> ( \<comment>\<open>add sub-tree starting from non-terminal\<close>
         do {
-          t \<leftarrow> build_tree' bs inp k' pre;
+          t \<leftarrow> build_tree' bs \<omega> k' pre;
           case t of
             Branch N ts \<Rightarrow>
               do {
-                t \<leftarrow> build_tree' bs inp k red;
+                t \<leftarrow> build_tree' bs \<omega> k red;
                 Some (Branch N (ts @ [t]))
               }
           | _ \<Rightarrow> undefined \<comment>\<open>impossible case\<close>
@@ -746,57 +754,57 @@ partial_function (option) build_tree' :: "'a bins \<Rightarrow> 'a sentence \<Ri
 declare build_tree'.simps [code]
 
 definition build_tree :: "'a cfg \<Rightarrow> 'a sentence \<Rightarrow> 'a bins \<Rightarrow> 'a tree option" where
-  "build_tree cfg inp bs = (
+  "build_tree \<G> \<omega> bs = (
     let k = length bs - 1 in (
-    case filter_with_index (\<lambda>x. is_finished cfg inp x) (items (bs!k)) of
+    case filter_with_index (\<lambda>x. is_finished \<G> \<omega> x) (items (bs!k)) of
       [] \<Rightarrow> None
-    | (_, i)#_ \<Rightarrow> build_tree' bs inp k i
+    | (_, i)#_ \<Rightarrow> build_tree' bs \<omega> k i
   ))"
 
 lemma build_tree'_simps[simp]:
-  "e = bs!k!i \<Longrightarrow> pointer e = Null \<Longrightarrow> build_tree' bs inp k i = Some (Branch (item_rule_head (item e)) [])"
-  "e = bs!k!i \<Longrightarrow> pointer e = Pre pre \<Longrightarrow> build_tree' bs inp (k-1) pre = None \<Longrightarrow>
-   build_tree' bs inp k i = None"
-  "e = bs!k!i \<Longrightarrow> pointer e = Pre pre \<Longrightarrow> build_tree' bs inp (k-1) pre = Some (Branch N ts) \<Longrightarrow>
-   build_tree' bs inp k i = Some (Branch N (ts @ [Leaf (inp!(k-1))]))"
-  "e = bs!k!i \<Longrightarrow> pointer e = Pre pre \<Longrightarrow> build_tree' bs inp (k-1) pre = Some (Leaf a) \<Longrightarrow>
-   build_tree' bs inp k i = undefined"
-  "e = bs!k!i \<Longrightarrow> pointer e = PreRed (k', pre, red) reds \<Longrightarrow> build_tree' bs inp k' pre = None \<Longrightarrow>
-   build_tree' bs inp k i = None"
-  "e = bs!k!i \<Longrightarrow> pointer e = PreRed (k', pre, red) reds \<Longrightarrow> build_tree' bs inp k' pre = Some (Branch N ts) \<Longrightarrow>
-   build_tree' bs inp k red = None \<Longrightarrow> build_tree' bs inp k i = None"
-  "e = bs!k!i \<Longrightarrow> pointer e = PreRed (k', pre, red) reds \<Longrightarrow> build_tree' bs inp k' pre = Some (Leaf a) \<Longrightarrow>
-   build_tree' bs inp k i = undefined"
-  "e = bs!k!i \<Longrightarrow> pointer e = PreRed (k', pre, red) reds \<Longrightarrow> build_tree' bs inp k' pre = Some (Branch N ts) \<Longrightarrow>
-   build_tree' bs inp k red = Some t \<Longrightarrow>
-   build_tree' bs inp k i = Some (Branch N (ts @ [t]))"
+  "e = bs!k!i \<Longrightarrow> pointer e = Null \<Longrightarrow> build_tree' bs \<omega> k i = Some (Branch (item_rule_head (item e)) [])"
+  "e = bs!k!i \<Longrightarrow> pointer e = Pre pre \<Longrightarrow> build_tree' bs \<omega> (k-1) pre = None \<Longrightarrow>
+   build_tree' bs \<omega> k i = None"
+  "e = bs!k!i \<Longrightarrow> pointer e = Pre pre \<Longrightarrow> build_tree' bs \<omega> (k-1) pre = Some (Branch N ts) \<Longrightarrow>
+   build_tree' bs \<omega> k i = Some (Branch N (ts @ [Leaf (\<omega>!(k-1))]))"
+  "e = bs!k!i \<Longrightarrow> pointer e = Pre pre \<Longrightarrow> build_tree' bs \<omega> (k-1) pre = Some (Leaf a) \<Longrightarrow>
+   build_tree' bs \<omega> k i = undefined"
+  "e = bs!k!i \<Longrightarrow> pointer e = PreRed (k', pre, red) reds \<Longrightarrow> build_tree' bs \<omega> k' pre = None \<Longrightarrow>
+   build_tree' bs \<omega> k i = None"
+  "e = bs!k!i \<Longrightarrow> pointer e = PreRed (k', pre, red) reds \<Longrightarrow> build_tree' bs \<omega> k' pre = Some (Branch N ts) \<Longrightarrow>
+   build_tree' bs \<omega> k red = None \<Longrightarrow> build_tree' bs \<omega> k i = None"
+  "e = bs!k!i \<Longrightarrow> pointer e = PreRed (k', pre, red) reds \<Longrightarrow> build_tree' bs \<omega> k' pre = Some (Leaf a) \<Longrightarrow>
+   build_tree' bs \<omega> k i = undefined"
+  "e = bs!k!i \<Longrightarrow> pointer e = PreRed (k', pre, red) reds \<Longrightarrow> build_tree' bs \<omega> k' pre = Some (Branch N ts) \<Longrightarrow>
+   build_tree' bs \<omega> k red = Some t \<Longrightarrow>
+   build_tree' bs \<omega> k i = Some (Branch N (ts @ [t]))"
   by (subst build_tree'.simps, simp)+
 
 definition wf_tree_input :: "('a bins \<times> 'a sentence \<times> nat \<times> nat) set" where
   "wf_tree_input = {
-    (bs, inp, k, i) | bs inp k i.
-      sound_ptrs inp bs \<and>
+    (bs, \<omega>, k, i) | bs \<omega> k i.
+      sound_ptrs \<omega> bs \<and>
       mono_red_ptr bs \<and>
       k < length bs \<and>
       i < length (bs!k)
   }"
 
 fun build_tree'_measure :: "('a bins \<times> 'a sentence \<times> nat \<times> nat) \<Rightarrow> nat" where
-  "build_tree'_measure (bs, inp, k, i) = foldl (+) 0 (map length (take k bs)) + i"
+  "build_tree'_measure (bs, \<omega>, k, i) = foldl (+) 0 (map length (take k bs)) + i"
 
 lemma wf_tree_input_pre:
-  assumes "(bs, inp, k, i) \<in> wf_tree_input"
+  assumes "(bs, \<omega>, k, i) \<in> wf_tree_input"
   assumes "e = bs!k!i" "pointer e = Pre pre"
-  shows "(bs, inp, (k-1), pre) \<in> wf_tree_input"
+  shows "(bs, \<omega>, (k-1), pre) \<in> wf_tree_input"
   using assms unfolding wf_tree_input_def
   apply (auto simp: sound_ptrs_def sound_pre_ptr_def)
   apply (metis nth_mem)
   done
 
 lemma wf_tree_input_prered_pre:
-  assumes "(bs, inp, k, i) \<in> wf_tree_input"
+  assumes "(bs, \<omega>, k, i) \<in> wf_tree_input"
   assumes "e = bs!k!i" "pointer e = PreRed (k', pre, red) ps"
-  shows "(bs, inp, k', pre) \<in> wf_tree_input"
+  shows "(bs, \<omega>, k', pre) \<in> wf_tree_input"
   using assms unfolding wf_tree_input_def
   apply (auto simp: sound_ptrs_def sound_prered_ptr_def)
   apply metis+
@@ -804,24 +812,24 @@ lemma wf_tree_input_prered_pre:
   by (metis nth_mem)
 
 lemma wf_tree_input_prered_red:
-  assumes "(bs, inp, k, i) \<in> wf_tree_input"
+  assumes "(bs, \<omega>, k, i) \<in> wf_tree_input"
   assumes "e = bs!k!i" "pointer e = PreRed (k', pre, red) ps"
-  shows "(bs, inp, k, red) \<in> wf_tree_input"
+  shows "(bs, \<omega>, k, red) \<in> wf_tree_input"
   using assms unfolding wf_tree_input_def
   apply (auto simp add: sound_ptrs_def sound_prered_ptr_def)
   apply (metis nth_mem)+
   done
 
 lemma build_tree'_induct:
-  assumes "(bs, inp, k, i) \<in> wf_tree_input"
-  assumes "\<And>bs inp k i.
-    (\<And>e pre. e = bs!k!i \<Longrightarrow> pointer e = Pre pre \<Longrightarrow> P bs inp (k-1) pre) \<Longrightarrow>
-    (\<And>e k' pre red ps. e = bs!k!i \<Longrightarrow> pointer e = PreRed (k', pre, red) ps \<Longrightarrow> P bs inp k' pre) \<Longrightarrow>
-    (\<And>e k' pre red ps. e = bs!k!i \<Longrightarrow> pointer e = PreRed (k', pre, red) ps \<Longrightarrow> P bs inp k red) \<Longrightarrow>
-    P bs inp k i" 
-  shows "P bs inp k i"
+  assumes "(bs, \<omega>, k, i) \<in> wf_tree_input"
+  assumes "\<And>bs \<omega> k i.
+    (\<And>e pre. e = bs!k!i \<Longrightarrow> pointer e = Pre pre \<Longrightarrow> P bs \<omega> (k-1) pre) \<Longrightarrow>
+    (\<And>e k' pre red ps. e = bs!k!i \<Longrightarrow> pointer e = PreRed (k', pre, red) ps \<Longrightarrow> P bs \<omega> k' pre) \<Longrightarrow>
+    (\<And>e k' pre red ps. e = bs!k!i \<Longrightarrow> pointer e = PreRed (k', pre, red) ps \<Longrightarrow> P bs \<omega> k red) \<Longrightarrow>
+    P bs \<omega> k i" 
+  shows "P bs \<omega> k i"
   using assms(1)
-proof (induction n\<equiv>"build_tree'_measure (bs, inp, k, i)" arbitrary: k i rule: nat_less_induct)
+proof (induction n\<equiv>"build_tree'_measure (bs, \<omega>, k, i)" arbitrary: k i rule: nat_less_induct)
   case 1
   obtain e where entry: "e = bs!k!i"
     by simp
@@ -838,7 +846,7 @@ proof (induction n\<equiv>"build_tree'_measure (bs, inp, k, i)" arbitrary: k i r
     case Pre
     then obtain pre where pre: "pointer e = Pre pre"
       by blast
-    define n where n: "n = build_tree'_measure (bs, inp, (k-1), pre)"
+    define n where n: "n = build_tree'_measure (bs, \<omega>, (k-1), pre)"
     have "0 < k" "pre < length (bs!(k-1))"
       using 1(2) entry pre unfolding wf_tree_input_def sound_ptrs_def sound_pre_ptr_def
       by (smt (verit) mem_Collect_eq nth_mem prod.inject)+
@@ -851,9 +859,9 @@ proof (induction n\<equiv>"build_tree'_measure (bs, inp, k, i)" arbitrary: k i r
       by simp
     also have "... > 0"
       using \<open>pre < length (bs!(k-1))\<close> by auto
-    finally have "build_tree'_measure (bs, inp, k, i) - build_tree'_measure (bs, inp, (k-1), pre) > 0"
+    finally have "build_tree'_measure (bs, \<omega>, k, i) - build_tree'_measure (bs, \<omega>, (k-1), pre) > 0"
       by simp
-    hence "P bs inp (k-1) pre"
+    hence "P bs \<omega> (k-1) pre"
       using 1 n wf_tree_input_pre entry pre zero_less_diff by blast
     thus ?thesis
       using assms(2) entry pre pointer.distinct(5) pointer.inject(1) by presburger
@@ -870,7 +878,7 @@ proof (induction n\<equiv>"build_tree'_measure (bs, inp, k, i)" arbitrary: k i r
       using 1(2) entry prered unfolding wf_tree_input_def mono_red_ptr_def by blast
     have "k < length bs" "i < length (bs!k)"
       using 1(2) unfolding wf_tree_input_def by blast+
-    define n_pre where n_pre: "n_pre = build_tree'_measure (bs, inp, k', pre)"
+    define n_pre where n_pre: "n_pre = build_tree'_measure (bs, \<omega>, k', pre)"
     have "0 < length (bs!k') + i - pre"
       by (simp add: \<open>pre < length (bs!k')\<close> add.commute trans_less_add2)
     also have "... = foldl (+) 0 (map length (take k' bs)) + length (bs!k') + i - (foldl (+) 0 (map length (take k' bs)) + pre)"
@@ -879,14 +887,14 @@ proof (induction n\<equiv>"build_tree'_measure (bs, inp, k, i)" arbitrary: k i r
       using foldl_add_nth_ge[of k' k' bs 0] \<open>k < length bs\<close> \<open>k' < k\<close> by simp
     also have "... \<le> foldl (+) 0 (map length (take k bs)) + i - (foldl (+) 0 (map length (take k' bs)) + pre)"
       using foldl_take_mono by (metis Suc_eq_plus1 Suc_leI \<open>k' < k\<close> add.commute add_le_cancel_left diff_le_mono)
-    finally have "build_tree'_measure (bs, inp, k, i) - build_tree'_measure (bs, inp, k', pre) > 0"
+    finally have "build_tree'_measure (bs, \<omega>, k, i) - build_tree'_measure (bs, \<omega>, k', pre) > 0"
       by simp
-    hence x: "P bs inp k' pre"
+    hence x: "P bs \<omega> k' pre"
       using 1(1) zero_less_diff by (metis "1.prems" entry prered wf_tree_input_prered_pre)
-    define n_red where n_red: "n_red = build_tree'_measure (bs, inp, k, red)"
-    have "build_tree'_measure (bs, inp, k, i) - build_tree'_measure (bs, inp, k, red) > 0"
+    define n_red where n_red: "n_red = build_tree'_measure (bs, \<omega>, k, red)"
+    have "build_tree'_measure (bs, \<omega>, k, i) - build_tree'_measure (bs, \<omega>, k, red) > 0"
       using \<open>red < i\<close> by simp
-    hence y: "P bs inp k red"
+    hence y: "P bs \<omega> k red"
       using "1.hyps" "1.prems" entry prered wf_tree_input_prered_red zero_less_diff by blast
     show ?thesis
       using assms(2) x y entry prered 
@@ -895,12 +903,12 @@ proof (induction n\<equiv>"build_tree'_measure (bs, inp, k, i)" arbitrary: k i r
 qed
 
 lemma build_tree'_termination:
-  assumes "(bs, inp, k, i) \<in> wf_tree_input"
-  shows "\<exists>N ts. build_tree' bs inp k i = Some (Branch N ts)"
+  assumes "(bs, \<omega>, k, i) \<in> wf_tree_input"
+  shows "\<exists>N ts. build_tree' bs \<omega> k i = Some (Branch N ts)"
 proof -
-  have "\<exists>N ts. build_tree' bs inp k i = Some (Branch N ts)"
+  have "\<exists>N ts. build_tree' bs \<omega> k i = Some (Branch N ts)"
     apply (induction rule: build_tree'_induct[OF assms(1)])
-    subgoal premises IH for bs inp k i
+    subgoal premises IH for bs \<omega> k i
     proof -
       define e where entry: "e = bs!k!i"
       consider (Null) "pointer e = Null"
@@ -916,9 +924,9 @@ proof -
         case Pre
         then obtain pre where pre: "pointer e = Pre pre"
           by blast
-        obtain N ts where Nts: "build_tree' bs inp (k-1) pre = Some (Branch N ts)"
+        obtain N ts where Nts: "build_tree' bs \<omega> (k-1) pre = Some (Branch N ts)"
           using IH(1) entry pre by blast
-        have "build_tree' bs inp k i = Some (Branch N (ts @ [Leaf (inp!(k-1))]))"
+        have "build_tree' bs \<omega> k i = Some (Branch N (ts @ [Leaf (\<omega>!(k-1))]))"
           using build_tree'_simps(3) entry pre Nts by simp         
         thus ?thesis
           by simp
@@ -926,11 +934,11 @@ proof -
         case PreRed
         then obtain k' pre red ps where prered: "pointer e = PreRed (k', pre, red) ps"
           by blast
-        then obtain N ts where Nts: "build_tree' bs inp k' pre = Some (Branch N ts)"
+        then obtain N ts where Nts: "build_tree' bs \<omega> k' pre = Some (Branch N ts)"
           using IH(2) entry prered by blast
-        obtain t_red where t_red: "build_tree' bs inp k red = Some t_red"
+        obtain t_red where t_red: "build_tree' bs \<omega> k red = Some t_red"
           using IH(3) entry prered Nts by (metis option.exhaust)
-        have "build_tree' bs inp k i = Some (Branch N (ts @ [t_red]))"
+        have "build_tree' bs \<omega> k i = Some (Branch N (ts @ [t_red]))"
           using build_tree'_simps(8) entry prered Nts t_red by auto
         thus ?thesis
           by blast
@@ -942,16 +950,16 @@ proof -
 qed
 
 lemma wf_item_tree_build_tree':
-  assumes "(bs, inp, k, i) \<in> wf_tree_input"
-  assumes "wf_bins cfg inp bs"
+  assumes "(bs, \<omega>, k, i) \<in> wf_tree_input"
+  assumes "wf_bins \<G> \<omega> bs"
   assumes "k < length bs" "i < length (bs!k)"
-  assumes "build_tree' bs inp k i = Some t"
-  shows "wf_item_tree cfg (item (bs!k!i)) t"
+  assumes "build_tree' bs \<omega> k i = Some t"
+  shows "wf_item_tree \<G> (item (bs!k!i)) t"
 proof -
-  have "wf_item_tree cfg (item (bs!k!i)) t"
+  have "wf_item_tree \<G> (item (bs!k!i)) t"
     using assms
     apply (induction arbitrary: t rule: build_tree'_induct[OF assms(1)])
-    subgoal premises prems for bs inp k i t
+    subgoal premises prems for bs \<omega> k i t
     proof -
       define e where entry: "e = bs!k!i"
       consider (Null) "pointer e = Null"
@@ -961,11 +969,11 @@ proof -
       thus ?thesis
       proof cases
         case Null
-        hence "build_tree' bs inp k i = Some (Branch (item_rule_head (item e)) [])"
+        hence "build_tree' bs \<omega> k i = Some (Branch (item_rule_head (item e)) [])"
           using entry by simp
         have simp: "t = Branch (item_rule_head (item e)) []"
           using build_tree'_simps(1) Null prems(8) entry by simp
-        have "sound_ptrs inp bs"
+        have "sound_ptrs \<omega> bs"
           using prems(4) unfolding wf_tree_input_def by blast
         hence "predicts (item e)"
           using Null prems(6,7) nth_mem entry unfolding sound_ptrs_def sound_null_ptr_def by blast
@@ -977,36 +985,36 @@ proof -
         case Pre
         then obtain pre where pre: "pointer e = Pre pre"
           by blast
-        obtain N ts where Nts: "build_tree' bs inp (k-1) pre = Some (Branch N ts)"
+        obtain N ts where Nts: "build_tree' bs \<omega> (k-1) pre = Some (Branch N ts)"
           using build_tree'_termination entry pre prems(4) wf_tree_input_pre by blast
-        have simp: "build_tree' bs inp k i = Some (Branch N (ts @ [Leaf (inp!(k-1))]))"
+        have simp: "build_tree' bs \<omega> k i = Some (Branch N (ts @ [Leaf (\<omega>!(k-1))]))"
           using build_tree'_simps(3) entry pre Nts by simp
-        have "sound_ptrs inp bs"
+        have "sound_ptrs \<omega> bs"
           using prems(4) unfolding wf_tree_input_def by blast
         hence "pre < length (bs!(k-1))"
           using entry pre prems(6,7) unfolding sound_ptrs_def sound_pre_ptr_def by (metis nth_mem)
         moreover have "k-1 < length bs"
           by (simp add: prems(6) less_imp_diff_less)
-        ultimately have IH: "wf_item_tree cfg (item (bs!(k-1)!pre)) (Branch N ts)"
+        ultimately have IH: "wf_item_tree \<G> (item (bs!(k-1)!pre)) (Branch N ts)"
           using prems(1,2,4,5) entry pre Nts by (meson wf_tree_input_pre)
-        have scans: "scans inp k (item (bs!(k-1)!pre)) (item e)"
-          using entry pre prems(6-7) \<open>sound_ptrs inp bs\<close> unfolding sound_ptrs_def sound_pre_ptr_def by simp
+        have scans: "scans \<omega> k (item (bs!(k-1)!pre)) (item e)"
+          using entry pre prems(6-7) \<open>sound_ptrs \<omega> bs\<close> unfolding sound_ptrs_def sound_pre_ptr_def by simp
         hence *: 
           "item_rule_head (item (bs!(k-1)!pre)) = item_rule_head (item e)"
           "item_rule_body (item (bs!(k-1)!pre)) = item_rule_body (item e)"
           "item_dot (item (bs!(k-1)!pre)) + 1 = item_dot (item e)"
-          "next_symbol (item (bs!(k-1)!pre)) = Some (inp!(k-1))"
+          "next_symbol (item (bs!(k-1)!pre)) = Some (\<omega>!(k-1))"
           unfolding scans_def inc_item_def by (simp_all add: item_rule_head_def item_rule_body_def)
-        have "map root_tree (ts @ [Leaf (inp!(k-1))]) = map root_tree ts @ [inp!(k-1)]"
+        have "map root_tree (ts @ [Leaf (\<omega>!(k-1))]) = map root_tree ts @ [\<omega>!(k-1)]"
           by simp
-        also have "... = take (item_dot (item (bs!(k-1)!pre))) (item_rule_body (item (bs!(k-1)!pre))) @ [inp!(k-1)]"
+        also have "... = take (item_dot (item (bs!(k-1)!pre))) (item_rule_body (item (bs!(k-1)!pre))) @ [\<omega>!(k-1)]"
           using IH by simp
-        also have "... = take (item_dot (item (bs!(k-1)!pre))) (item_rule_body (item e)) @ [inp!(k-1)]"
+        also have "... = take (item_dot (item (bs!(k-1)!pre))) (item_rule_body (item e)) @ [\<omega>!(k-1)]"
           using *(2) by simp
         also have "... = take (item_dot (item e)) (item_rule_body (item e))"
           using *(2-4) by (auto simp: next_symbol_def is_complete_def split: if_splits; metis leI take_Suc_conv_app_nth)
-        finally have "map root_tree (ts @ [Leaf (inp!(k-1))]) = take (item_dot (item e)) (item_rule_body (item e))" .
-        hence "wf_item_tree cfg (item e) (Branch N (ts @ [Leaf (inp!(k-1))]))"
+        finally have "map root_tree (ts @ [Leaf (\<omega>!(k-1))]) = take (item_dot (item e)) (item_rule_body (item e))" .
+        hence "wf_item_tree \<G> (item e) (Branch N (ts @ [Leaf (\<omega>!(k-1))]))"
           using IH *(1) by simp
         thus ?thesis
           using entry prems(8) simp by auto
@@ -1014,19 +1022,19 @@ proof -
         case PreRed
         then obtain k' pre red ps where prered: "pointer e = PreRed (k', pre, red) ps"
           by blast
-        obtain N ts where Nts: "build_tree' bs inp k' pre = Some (Branch N ts)"
+        obtain N ts where Nts: "build_tree' bs \<omega> k' pre = Some (Branch N ts)"
           using build_tree'_termination entry prems(4) prered wf_tree_input_prered_pre by blast
-        obtain N_red ts_red where Nts_red: "build_tree' bs inp k red = Some (Branch N_red ts_red)"
+        obtain N_red ts_red where Nts_red: "build_tree' bs \<omega> k red = Some (Branch N_red ts_red)"
           using build_tree'_termination entry prems(4) prered wf_tree_input_prered_red by blast
-        have simp: "build_tree' bs inp k i = Some (Branch N (ts @ [Branch N_red ts_red]))"
+        have simp: "build_tree' bs \<omega> k i = Some (Branch N (ts @ [Branch N_red ts_red]))"
           using build_tree'_simps(8) entry prered Nts Nts_red by auto
-        have "sound_ptrs inp bs"
+        have "sound_ptrs \<omega> bs"
           using prems(4) wf_tree_input_def by fastforce
         have bounds: "k' < k" "pre < length (bs!k')" "red < length (bs!k)"
-          using prered entry prems(6,7) \<open>sound_ptrs inp bs\<close>
+          using prered entry prems(6,7) \<open>sound_ptrs \<omega> bs\<close>
           unfolding sound_prered_ptr_def sound_ptrs_def by fastforce+
         have completes: "completes k (item (bs!k'!pre)) (item e) (item (bs!k!red))"
-          using prered entry prems(6,7) \<open>sound_ptrs inp bs\<close>
+          using prered entry prems(6,7) \<open>sound_ptrs \<omega> bs\<close>
           unfolding sound_ptrs_def sound_prered_ptr_def by fastforce
         have *: 
           "item_rule_head (item (bs!k'!pre)) = item_rule_head (item e)"
@@ -1036,13 +1044,13 @@ proof -
           "is_complete (item (bs!k!red))"
           using completes unfolding completes_def inc_item_def
           by (auto simp: item_rule_head_def item_rule_body_def is_complete_def)
-        have "(bs, inp, k', pre) \<in> wf_tree_input"
+        have "(bs, \<omega>, k', pre) \<in> wf_tree_input"
           using wf_tree_input_prered_pre[OF prems(4) entry prered] by blast
-        hence IH_pre: "wf_item_tree cfg (item (bs!k'!pre)) (Branch N ts)"
+        hence IH_pre: "wf_item_tree \<G> (item (bs!k'!pre)) (Branch N ts)"
           using prems(2)[OF entry prered _ prems(5)] Nts bounds(1,2) order_less_trans prems(6) by blast
-        have "(bs, inp, k, red) \<in> wf_tree_input"
+        have "(bs, \<omega>, k, red) \<in> wf_tree_input"
           using wf_tree_input_prered_red[OF prems(4) entry prered] by blast   
-        hence IH_r: "wf_item_tree cfg (item (bs!k!red)) (Branch N_red ts_red)"
+        hence IH_r: "wf_item_tree \<G> (item (bs!k!red)) (Branch N_red ts_red)"
           using bounds(3) entry prems(3,5,6) prered Nts_red by blast
         have "map root_tree (ts @ [Branch N_red ts_red]) = map root_tree ts @ [root_tree (Branch N_red ts)]"
           by simp
@@ -1053,17 +1061,17 @@ proof -
         also have "... = take (item_dot (item e)) (item_rule_body (item e))"
           using * by (auto simp: next_symbol_def is_complete_def split: if_splits; metis leI take_Suc_conv_app_nth)
         finally have roots: "map root_tree (ts @ [Branch N_red ts]) = take (item_dot (item e)) (item_rule_body (item e))" by simp
-        have "wf_item cfg inp (item (bs!k!red))"
+        have "wf_item \<G> \<omega> (item (bs!k!red))"
           using prems(5,6) bounds(3) unfolding wf_bins_def wf_bin_def wf_bin_items_def by (auto simp: items_def) 
         moreover have "N_red = item_rule_head (item (bs!k!red))"
           using IH_r by fastforce
         moreover have "map root_tree ts_red = item_rule_body (item (bs!k!red))"
           using IH_r *(5) by (auto simp: is_complete_def)
-        ultimately have "\<exists>r \<in> set (\<RR> cfg). N_red = rule_head r \<and> map root_tree ts_red = rule_body r"
+        ultimately have "\<exists>r \<in> set (\<RR> \<G>). N_red = rule_head r \<and> map root_tree ts_red = rule_body r"
           unfolding wf_item_def item_rule_body_def item_rule_head_def by blast
-        hence "wf_rule_tree cfg (Branch N_red ts_red)"
+        hence "wf_rule_tree \<G> (Branch N_red ts_red)"
           using IH_r by simp
-        hence "wf_item_tree cfg (item (bs!k!i)) (Branch N (ts @ [Branch N_red ts_red]))"
+        hence "wf_item_tree \<G> (item (bs!k!i)) (Branch N (ts @ [Branch N_red ts_red]))"
           using "*"(1) roots IH_pre entry by simp
         thus ?thesis
           using Nts_red prems(8) simp by auto
@@ -1075,16 +1083,16 @@ proof -
 qed
 
 lemma wf_yield_tree_build_tree':
-  assumes "(bs, inp, k, i) \<in> wf_tree_input"
-  assumes "wf_bins cfg inp bs"
-  assumes "k < length bs" "i < length (bs!k)" "k \<le> length inp"
-  assumes "build_tree' bs inp k i = Some t"
-  shows "wf_yield_tree inp (item (bs!k!i)) t"
+  assumes "(bs, \<omega>, k, i) \<in> wf_tree_input"
+  assumes "wf_bins \<G> \<omega> bs"
+  assumes "k < length bs" "i < length (bs!k)" "k \<le> length \<omega>"
+  assumes "build_tree' bs \<omega> k i = Some t"
+  shows "wf_yield_tree \<omega> (item (bs!k!i)) t"
 proof -
-  have "wf_yield_tree inp (item (bs!k!i)) t"
+  have "wf_yield_tree \<omega> (item (bs!k!i)) t"
     using assms
     apply (induction arbitrary: t rule: build_tree'_induct[OF assms(1)])
-    subgoal premises prems for bs inp k i t
+    subgoal premises prems for bs \<omega> k i t
     proof -
       define e where entry: "e = bs!k!i"
       consider (Null) "pointer e = Null"
@@ -1094,11 +1102,11 @@ proof -
       thus ?thesis
       proof cases
         case Null
-        hence "build_tree' bs inp k i = Some (Branch (item_rule_head (item e)) [])"
+        hence "build_tree' bs \<omega> k i = Some (Branch (item_rule_head (item e)) [])"
           using entry by simp
         have simp: "t = Branch (item_rule_head (item e)) []"
           using build_tree'_simps(1) Null prems(9) entry by simp
-        have "sound_ptrs inp bs"
+        have "sound_ptrs \<omega> bs"
           using prems(4) unfolding wf_tree_input_def by blast
         hence "predicts (item e)"
           using Null prems(6,7) nth_mem entry unfolding sound_ptrs_def sound_null_ptr_def by blast
@@ -1108,40 +1116,40 @@ proof -
         case Pre
         then obtain pre where pre: "pointer e = Pre pre"
           by blast
-        obtain N ts where Nts: "build_tree' bs inp (k-1) pre = Some (Branch N ts)"
+        obtain N ts where Nts: "build_tree' bs \<omega> (k-1) pre = Some (Branch N ts)"
           using build_tree'_termination entry pre prems(4) wf_tree_input_pre by blast
-        have simp: "build_tree' bs inp k i = Some (Branch N (ts @ [Leaf (inp!(k-1))]))"
+        have simp: "build_tree' bs \<omega> k i = Some (Branch N (ts @ [Leaf (\<omega>!(k-1))]))"
           using build_tree'_simps(3) entry pre Nts by simp
-        have "sound_ptrs inp bs"
+        have "sound_ptrs \<omega> bs"
           using prems(4) unfolding wf_tree_input_def by blast
         hence bounds: "k > 0" "pre < length (bs!(k-1))"
           using entry pre prems(6,7) unfolding sound_ptrs_def sound_pre_ptr_def by (metis nth_mem)+
         moreover have "k-1 < length bs"
           by (simp add: prems(6) less_imp_diff_less)
-        ultimately have IH: "wf_yield_tree inp (item (bs!(k-1)!pre)) (Branch N ts)"
+        ultimately have IH: "wf_yield_tree \<omega> (item (bs!(k-1)!pre)) (Branch N ts)"
           using prems(1) entry pre Nts wf_tree_input_pre prems(4,5,8) by fastforce
-        have scans: "scans inp k (item (bs!(k-1)!pre)) (item e)"
-          using entry pre prems(6-7) \<open>sound_ptrs inp bs\<close> unfolding sound_ptrs_def sound_pre_ptr_def by simp
+        have scans: "scans \<omega> k (item (bs!(k-1)!pre)) (item e)"
+          using entry pre prems(6-7) \<open>sound_ptrs \<omega> bs\<close> unfolding sound_ptrs_def sound_pre_ptr_def by simp
         have wf: 
           "item_origin (item (bs!(k-1)!pre)) \<le> item_end (item (bs!(k-1)!pre))"
           "item_end (item (bs!(k-1)!pre)) = k-1"
           "item_end (item e) = k"
           using entry prems(5,6,7) bounds unfolding wf_bins_def wf_bin_def wf_bin_items_def items_def wf_item_def
           by (auto, meson less_imp_diff_less nth_mem)
-        have "yield_tree (Branch N (ts @ [Leaf (inp!(k-1))])) = concat (map yield_tree (ts @ [Leaf (inp!(k-1))]))"
+        have "yield_tree (Branch N (ts @ [Leaf (\<omega>!(k-1))])) = concat (map yield_tree (ts @ [Leaf (\<omega>!(k-1))]))"
           by simp
-        also have "... = concat (map yield_tree ts) @ [inp!(k-1)]"
+        also have "... = concat (map yield_tree ts) @ [\<omega>!(k-1)]"
           by simp
-        also have "... = slice (item_origin (item (bs!(k-1)!pre))) (item_end (item (bs!(k-1)!pre))) inp @ [inp!(k-1)]"
+        also have "... = slice (item_origin (item (bs!(k-1)!pre))) (item_end (item (bs!(k-1)!pre))) \<omega> @ [\<omega>!(k-1)]"
           using IH by (simp add: wf_yield_tree_def)
-        also have "... = slice (item_origin (item (bs!(k-1)!pre))) (item_end (item (bs!(k-1)!pre)) + 1) inp"
+        also have "... = slice (item_origin (item (bs!(k-1)!pre))) (item_end (item (bs!(k-1)!pre)) + 1) \<omega>"
           using slice_append_nth wf \<open>k > 0\<close> prems(8)
           by (metis diff_less le_eq_less_or_eq less_imp_diff_less less_numeral_extra(1))
-        also have "... = slice (item_origin (item e)) (item_end (item (bs!(k-1)!pre)) + 1) inp"
+        also have "... = slice (item_origin (item e)) (item_end (item (bs!(k-1)!pre)) + 1) \<omega>"
           using scans unfolding scans_def inc_item_def by simp
-        also have "... = slice (item_origin (item e)) k inp"
+        also have "... = slice (item_origin (item e)) k \<omega>"
           using scans wf unfolding scans_def by (metis Suc_diff_1 Suc_eq_plus1 bounds(1))
-        also have "... = slice (item_origin (item e)) (item_end (item e)) inp"
+        also have "... = slice (item_origin (item e)) (item_end (item e)) \<omega>"
           using wf by auto
         finally show ?thesis
           using wf_yield_tree_def entry prems(9) simp by force
@@ -1149,28 +1157,28 @@ proof -
         case PreRed
         then obtain k' pre red ps where prered: "pointer e = PreRed (k', pre, red) ps"
           by blast
-        obtain N ts where Nts: "build_tree' bs inp k' pre = Some (Branch N ts)"
+        obtain N ts where Nts: "build_tree' bs \<omega> k' pre = Some (Branch N ts)"
           using build_tree'_termination entry prems(4) prered wf_tree_input_prered_pre by blast
-        obtain N_red ts_red where Nts_red: "build_tree' bs inp k red = Some (Branch N_red ts_red)"
+        obtain N_red ts_red where Nts_red: "build_tree' bs \<omega> k red = Some (Branch N_red ts_red)"
           using build_tree'_termination entry prems(4) prered wf_tree_input_prered_red by blast
-        have simp: "build_tree' bs inp k i = Some (Branch N (ts @ [Branch N_red ts_red]))"
+        have simp: "build_tree' bs \<omega> k i = Some (Branch N (ts @ [Branch N_red ts_red]))"
           using build_tree'_simps(8) entry prered Nts Nts_red by auto
-        have "sound_ptrs inp bs"
+        have "sound_ptrs \<omega> bs"
           using prems(4) wf_tree_input_def by fastforce
         have bounds: "k' < k" "pre < length (bs!k')" "red < length (bs!k)"
-          using prered entry prems(6,7) \<open>sound_ptrs inp bs\<close>
+          using prered entry prems(6,7) \<open>sound_ptrs \<omega> bs\<close>
           unfolding sound_ptrs_def sound_prered_ptr_def by fastforce+
         have completes: "completes k (item (bs!k'!pre)) (item e) (item (bs!k!red))"
-          using prered entry prems(6,7) \<open>sound_ptrs inp bs\<close>
+          using prered entry prems(6,7) \<open>sound_ptrs \<omega> bs\<close>
           unfolding sound_ptrs_def sound_prered_ptr_def by fastforce
-        have "(bs, inp, k', pre) \<in> wf_tree_input"
+        have "(bs, \<omega>, k', pre) \<in> wf_tree_input"
           using wf_tree_input_prered_pre[OF prems(4) entry prered] by blast
-        hence IH_pre: "wf_yield_tree inp (item (bs!k'!pre)) (Branch N ts)"
+        hence IH_pre: "wf_yield_tree \<omega> (item (bs!k'!pre)) (Branch N ts)"
           using prems(2)[OF entry prered _ prems(5)] Nts bounds(1,2) prems(6-8)
           by (meson dual_order.strict_trans1 nat_less_le)
-        have "(bs, inp, k, red) \<in> wf_tree_input"
+        have "(bs, \<omega>, k, red) \<in> wf_tree_input"
           using wf_tree_input_prered_red[OF prems(4) entry prered] by blast
-        hence IH_r: "wf_yield_tree inp (item (bs!k!red)) (Branch N_red ts_red)"
+        hence IH_r: "wf_yield_tree \<omega> (item (bs!k!red)) (Branch N_red ts_red)"
           using bounds(3) entry prems(3,5,6,8) prered Nts_red by blast
         have wf1: 
           "item_origin (item (bs!k'!pre)) \<le> item_end (item (bs!k'!pre))"
@@ -1185,14 +1193,14 @@ proof -
           by (simp add: Nts_red)
         also have "... = concat (map yield_tree ts) @ yield_tree (Branch N_red ts_red)"
           by simp
-        also have "... = slice (item_origin (item (bs!k'!pre))) (item_end (item (bs!k'!pre))) inp @ 
-          slice (item_origin (item (bs!k!red))) (item_end (item (bs!k!red))) inp"
+        also have "... = slice (item_origin (item (bs!k'!pre))) (item_end (item (bs!k'!pre))) \<omega> @ 
+          slice (item_origin (item (bs!k!red))) (item_end (item (bs!k!red))) \<omega>"
           using IH_pre IH_r by (simp add: wf_yield_tree_def)
-        also have "... = slice (item_origin (item (bs!k'!pre))) (item_end (item (bs!k!red))) inp"
+        also have "... = slice (item_origin (item (bs!k'!pre))) (item_end (item (bs!k!red))) \<omega>"
           using slice_concat wf1 completes_def completes by (metis (no_types, lifting))
-        also have "... = slice (item_origin (item e)) (item_end (item (bs!k!red))) inp"
+        also have "... = slice (item_origin (item e)) (item_end (item (bs!k!red))) \<omega>"
           using completes unfolding completes_def inc_item_def by simp
-        also have "... = slice (item_origin (item e)) (item_end (item e)) inp"
+        also have "... = slice (item_origin (item e)) (item_end (item e)) \<omega>"
           using wf2 entry by presburger
         finally show ?thesis
           using wf_yield_tree_def entry prems(9) simp by force
@@ -1204,107 +1212,107 @@ proof -
 qed
 
 theorem wf_rule_root_yield_tree_build_forest:
-  assumes "wf_bins cfg inp bs" "sound_ptrs inp bs" "mono_red_ptr bs" "length bs = length inp + 1"
-  assumes "build_tree cfg inp bs = Some t"
-  shows "wf_rule_tree cfg t \<and> root_tree t = \<SS> cfg \<and> yield_tree t = inp"
+  assumes "wf_bins \<G> \<omega> bs" "sound_ptrs \<omega> bs" "mono_red_ptr bs" "length bs = length \<omega> + 1"
+  assumes "build_tree \<G> \<omega> bs = Some t"
+  shows "wf_rule_tree \<G> t \<and> root_tree t = \<SS> \<G> \<and> yield_tree t = \<omega>"
 proof -
   let ?k = "length bs - 1"
-  define finished where finished_def: "finished = filter_with_index (is_finished cfg inp) (items (bs!?k))"
-  then obtain x i where *: "(x,i) \<in> set finished" "Some t = build_tree' bs inp ?k i"
+  define finished where finished_def: "finished = filter_with_index (is_finished \<G> \<omega>) (items (bs!?k))"
+  then obtain x i where *: "(x,i) \<in> set finished" "Some t = build_tree' bs \<omega> ?k i"
     using assms(5) unfolding finished_def build_tree_def by (auto simp: Let_def split: list.splits, presburger)
-  have k: "?k < length bs" "?k \<le> length inp"
+  have k: "?k < length bs" "?k \<le> length \<omega>"
     using assms(4) by simp_all
   have i: "i < length (bs!?k)"
     using index_filter_with_index_lt_length * items_def finished_def by (metis length_map)
   have x: "x = item (bs!?k!i)"
     using * i filter_with_index_nth items_def nth_map finished_def by metis
-  have finished: "is_finished cfg inp x"
+  have finished: "is_finished \<G> \<omega> x"
     using * filter_with_index_P finished_def by metis
-  have wf_trees_input: "(bs, inp, ?k, i) \<in> wf_tree_input"
+  have wf_trees_input: "(bs, \<omega>, ?k, i) \<in> wf_tree_input"
     unfolding wf_tree_input_def using assms(2,3) i k(1) by blast
-  hence wf_item_tree: "wf_item_tree cfg x t"
+  hence wf_item_tree: "wf_item_tree \<G> x t"
     using wf_item_tree_build_tree' assms(1,2) i k(1) x *(2) by metis
-  have wf_item: "wf_item cfg inp (item (bs!?k!i))"
+  have wf_item: "wf_item \<G> \<omega> (item (bs!?k!i))"
     using k(1) i assms(1) unfolding wf_bins_def wf_bin_def wf_bin_items_def by (simp add: items_def)
   obtain N ts where t: "t = Branch N ts"
     by (metis *(2) build_tree'_termination option.inject wf_trees_input)
   hence "N = item_rule_head x"
     "map root_tree ts = item_rule_body x"
     using finished wf_item_tree by (auto simp: is_finished_def is_complete_def)
-  hence "\<exists>r \<in> set (\<RR> cfg). N = rule_head r \<and> map root_tree ts = rule_body r"
+  hence "\<exists>r \<in> set (\<RR> \<G>). N = rule_head r \<and> map root_tree ts = rule_body r"
     using wf_item x unfolding wf_item_def item_rule_body_def item_rule_head_def by blast
-  hence wf_rule: "wf_rule_tree cfg t"
+  hence wf_rule: "wf_rule_tree \<G> t"
     using wf_item_tree t by simp
-  have root: "root_tree t = \<SS> cfg"
+  have root: "root_tree t = \<SS> \<G>"
     using finished t \<open>N = item_rule_head x\<close> by (auto simp: is_finished_def)
-  have "yield_tree t = slice (item_origin (item (bs!?k!i))) (item_end (item (bs!?k!i))) inp"
+  have "yield_tree t = slice (item_origin (item (bs!?k!i))) (item_end (item (bs!?k!i))) \<omega>"
     using k i assms(1) wf_trees_input wf_yield_tree_build_tree' wf_yield_tree_def *(2) by (metis (no_types, lifting))
-  hence yield: "yield_tree t = inp"
+  hence yield: "yield_tree t = \<omega>"
     using finished x unfolding is_finished_def by simp
   show ?thesis
     using * wf_rule root yield assms(4) unfolding build_tree_def by simp
 qed
 
 corollary wf_rule_root_yield_tree_build_tree_Earley\<^sub>L:
-  assumes "wf_\<G> cfg" "nonempty_derives cfg"
-  assumes "build_tree cfg inp (Earley\<^sub>L cfg inp) = Some t"
-  shows "wf_rule_tree cfg t \<and> root_tree t = \<SS> cfg \<and> yield_tree t = inp"
+  assumes "wf_\<G> \<G>" "nonempty_derives \<G>"
+  assumes "build_tree \<G> \<omega> (Earley\<^sub>L \<G> \<omega>) = Some t"
+  shows "wf_rule_tree \<G> t \<and> root_tree t = \<SS> \<G> \<and> yield_tree t = \<omega>"
   using assms wf_rule_root_yield_tree_build_forest wf_bins_Earley\<^sub>L sound_mono_ptrs_Earley\<^sub>L Earley\<^sub>L_def
     length_Earley\<^sub>L_bins length_bins_Init\<^sub>L by (metis nle_le)
 
 theorem correctness_build_tree_Earley\<^sub>L:
-  assumes "wf_\<G> cfg" "is_word cfg inp" "nonempty_derives cfg"
-  shows "(\<exists>t. build_tree cfg inp (Earley\<^sub>L cfg inp) = Some t) \<longleftrightarrow> derives cfg [\<SS> cfg] inp" (is "?L \<longleftrightarrow> ?R")
+  assumes "wf_\<G> \<G>" "is_word \<G> \<omega>" "nonempty_derives \<G>"
+  shows "(\<exists>t. build_tree \<G> \<omega> (Earley\<^sub>L \<G> \<omega>) = Some t) \<longleftrightarrow> derives \<G> [\<SS> \<G>] \<omega>" (is "?L \<longleftrightarrow> ?R")
 proof standard
   assume *: ?L
-  let ?k = "length (Earley\<^sub>L cfg inp) - 1"
-  define finished where finished_def: "finished = filter_with_index (is_finished cfg inp) (items ((Earley\<^sub>L cfg inp)!?k))"
-  then obtain t x i where *: "(x,i) \<in> set finished" "Some t = build_tree' (Earley\<^sub>L cfg inp) inp ?k i"
+  let ?k = "length (Earley\<^sub>L \<G> \<omega>) - 1"
+  define finished where finished_def: "finished = filter_with_index (is_finished \<G> \<omega>) (items ((Earley\<^sub>L \<G> \<omega>)!?k))"
+  then obtain t x i where *: "(x,i) \<in> set finished" "Some t = build_tree' (Earley\<^sub>L \<G> \<omega>) \<omega> ?k i"
     using * unfolding finished_def build_tree_def by (auto simp: Let_def split: list.splits, presburger)
-  have k: "?k < length (Earley\<^sub>L cfg inp)" "?k \<le> length inp"
+  have k: "?k < length (Earley\<^sub>L \<G> \<omega>)" "?k \<le> length \<omega>"
     by (simp_all add: Earley\<^sub>L_def assms(1))
-  have i: "i < length ((Earley\<^sub>L cfg inp) ! ?k)"
+  have i: "i < length ((Earley\<^sub>L \<G> \<omega>) ! ?k)"
     using index_filter_with_index_lt_length * items_def finished_def by (metis length_map)
-  have x: "x = item ((Earley\<^sub>L cfg inp)!?k!i)"
+  have x: "x = item ((Earley\<^sub>L \<G> \<omega>)!?k!i)"
     using * i filter_with_index_nth items_def nth_map finished_def by metis
-  have finished: "is_finished cfg inp x"
+  have finished: "is_finished \<G> \<omega> x"
     using * filter_with_index_P finished_def by metis
-  moreover have "x \<in> set (items ((Earley\<^sub>L cfg inp) ! ?k))"
+  moreover have "x \<in> set (items ((Earley\<^sub>L \<G> \<omega>) ! ?k))"
     using x by (auto simp: items_def; metis One_nat_def i imageI nth_mem)
-  ultimately have "(\<exists>x \<in> set (items ((Earley\<^sub>L cfg inp) ! length inp)). is_finished cfg inp x)"
-    by (metis assms(1) is_finished_def k(1) wf_bins_Earley\<^sub>L wf_bins_kth_bin)    
-  hence "earley_recognized_it (Earley\<^sub>L cfg inp) cfg inp"
-    using earley_recognized_it_def by blast
+  ultimately have "recognizing (bins (Earley\<^sub>L \<G> \<omega>)) \<G> \<omega>"
+    by (meson k(1) kth_bin_sub_bins recognizing_def subsetD)
   thus ?R
-    using correctness_list assms by blast
+    using correctness_Earley\<^sub>L assms by blast
 next
   assume *: ?R
-  let ?k = "length (Earley\<^sub>L cfg inp) - 1"
-  define finished where finished_def: "finished = filter_with_index (is_finished cfg inp) (items ((Earley\<^sub>L cfg inp)!?k))"
-  have "earley_recognized_it (Earley\<^sub>L cfg inp) cfg inp"
-    using assms * correctness_list by blast
-  moreover have "?k = length inp"
+  let ?k = "length (Earley\<^sub>L \<G> \<omega>) - 1"
+  define finished where finished_def: "finished = filter_with_index (is_finished \<G> \<omega>) (items ((Earley\<^sub>L \<G> \<omega>)!?k))"
+  have "recognizing (bins (Earley\<^sub>L \<G> \<omega>)) \<G> \<omega>"
+    using assms * correctness_Earley\<^sub>L by blast
+  moreover have "?k = length \<omega>"
     by (simp add: Earley\<^sub>L_def assms(1))
-  ultimately obtain x i xs where xis: "finished = (x,i)#xs"
-    using earley_recognized_it_def unfolding finished_def by (metis filter_with_index_nonempty neq_Nil_conv surj_pair)
-  hence simp: "build_tree cfg inp (Earley\<^sub>L cfg inp) = build_tree' (Earley\<^sub>L cfg inp) inp ?k i"
+  ultimately have "\<exists>x \<in> set (items ((Earley\<^sub>L \<G> \<omega>)!?k)). is_finished \<G> \<omega> x"
+    unfolding recognizing_def using assms(1) is_finished_def wf_bins_Earley\<^sub>L wf_item_in_kth_bin by metis
+  then obtain x i xs where xis: "finished = (x,i)#xs"
+    using filter_with_index_Ex_first by (metis finished_def)
+  hence simp: "build_tree \<G> \<omega> (Earley\<^sub>L \<G> \<omega>) = build_tree' (Earley\<^sub>L \<G> \<omega>) \<omega> ?k i"
     unfolding build_tree_def finished_def by auto
   have "(x,i) \<in> set finished"
     using xis by simp
-  hence "i < length ((Earley\<^sub>L cfg inp)!?k)"
+  hence "i < length ((Earley\<^sub>L \<G> \<omega>)!?k)"
     using index_filter_with_index_lt_length by (metis finished_def items_def length_map)
-  moreover have "?k < length (Earley\<^sub>L cfg inp)"
+  moreover have "?k < length (Earley\<^sub>L \<G> \<omega>)"
     by (simp add: Earley\<^sub>L_def assms(1))
-  ultimately have "(Earley\<^sub>L cfg inp, inp, ?k, i) \<in> wf_tree_input"
+  ultimately have "(Earley\<^sub>L \<G> \<omega>, \<omega>, ?k, i) \<in> wf_tree_input"
     unfolding wf_tree_input_def using sound_mono_ptrs_Earley\<^sub>L assms(1,3) by blast
-  then obtain N ts where "build_tree' (Earley\<^sub>L cfg inp) inp ?k i = Some (Branch N ts)"
+  then obtain N ts where "build_tree' (Earley\<^sub>L \<G> \<omega>) \<omega> ?k i = Some (Branch N ts)"
     using build_tree'_termination by blast
   thus ?L
     using simp by simp
 qed
 
 
-subsection \<open>Random those, map, map_option lemmas\<close>
+subsection \<open>those, map, map_option lemmas\<close>
 
 lemma those_map_exists:
   "Some ys = those (map f xs) \<Longrightarrow> y \<in> set ys \<Longrightarrow> \<exists>x. x \<in> set xs \<and> Some y \<in> set (map f xs)"
@@ -1328,10 +1336,10 @@ lemma map_Some_P:
   using assms by (induction xs) auto
 
 lemma those_map_FBranch_only:
-  assumes "g = (\<lambda>f. case f of FBranch N fss \<Rightarrow> Some (FBranch N (fss @ [[FLeaf (inp!(k-1))]])) | _ \<Rightarrow> None)"
+  assumes "g = (\<lambda>f. case f of FBranch N fss \<Rightarrow> Some (FBranch N (fss @ [[FLeaf (\<omega>!(k-1))]])) | _ \<Rightarrow> None)"
   assumes "Some fs = those (map g pres)" "f \<in> set fs"
   assumes "\<forall>f \<in> set pres. \<exists>N fss. f = FBranch N fss"
-  shows "\<exists>f_pre N fss. f = FBranch N (fss @ [[FLeaf (inp!(k-1))]]) \<and> f_pre = FBranch N fss \<and> f_pre \<in> set pres"
+  shows "\<exists>f_pre N fss. f = FBranch N (fss @ [[FLeaf (\<omega>!(k-1))]]) \<and> f_pre = FBranch N fss \<and> f_pre \<in> set pres"
   using assms
   apply (induction pres arbitrary: fs f)
   apply (auto)
@@ -1530,16 +1538,16 @@ proof (induction xs arbitrary: vs)
 qed simp
 
 partial_function (option) build_trees' :: "'a bins \<Rightarrow> 'a sentence \<Rightarrow> nat \<Rightarrow> nat \<Rightarrow> nat set \<Rightarrow> 'a forest list option" where
-  "build_trees' bs inp k i I = (
+  "build_trees' bs \<omega> k i I = (
     let e = bs!k!i in (
     case pointer e of
       Null \<Rightarrow> Some ([FBranch (item_rule_head (item e)) []]) \<comment>\<open>start building sub-trees\<close>
     | Pre pre \<Rightarrow> ( \<comment>\<open>add sub-trees starting from terminal\<close>
         do {
-          pres \<leftarrow> build_trees' bs inp (k-1) pre {pre};
+          pres \<leftarrow> build_trees' bs \<omega> (k-1) pre {pre};
           those (map (\<lambda>f.
             case f of
-              FBranch N fss \<Rightarrow> Some (FBranch N (fss @ [[FLeaf (inp!(k-1))]]))
+              FBranch N fss \<Rightarrow> Some (FBranch N (fss @ [[FLeaf (\<omega>!(k-1))]]))
             | _ \<Rightarrow> None  \<comment>\<open>impossible case\<close>
           ) pres)
         })
@@ -1548,8 +1556,8 @@ partial_function (option) build_trees' :: "'a bins \<Rightarrow> 'a sentence \<R
         let gs = group_by (\<lambda>(k', pre, red). (k', pre)) (\<lambda>(k', pre, red). red) ps' in
         map_option concat (those (map (\<lambda>((k', pre), reds).
           do {
-            pres \<leftarrow> build_trees' bs inp k' pre {pre};
-            rss \<leftarrow> those (map (\<lambda>red. build_trees' bs inp k red (I \<union> {red})) reds);
+            pres \<leftarrow> build_trees' bs \<omega> k' pre {pre};
+            rss \<leftarrow> those (map (\<lambda>red. build_trees' bs \<omega> k red (I \<union> {red})) reds);
             those (map (\<lambda>f.
               case f of
                 FBranch N fss \<Rightarrow> Some (FBranch N (fss @ [concat rss]))
@@ -1563,23 +1571,23 @@ partial_function (option) build_trees' :: "'a bins \<Rightarrow> 'a sentence \<R
 declare build_trees'.simps [code]
 
 definition build_trees :: "'a cfg \<Rightarrow> 'a sentence \<Rightarrow> 'a bins \<Rightarrow> 'a forest list option" where
-  "build_trees cfg inp bs = (
+  "build_trees \<G> \<omega> bs = (
     let k = length bs - 1 in
-    let finished = filter_with_index (\<lambda>x. is_finished cfg inp x) (items (bs!k)) in
-    map_option concat (those (map (\<lambda>(_, i). build_trees' bs inp k i {i}) finished))
+    let finished = filter_with_index (\<lambda>x. is_finished \<G> \<omega> x) (items (bs!k)) in
+    map_option concat (those (map (\<lambda>(_, i). build_trees' bs \<omega> k i {i}) finished))
   )"
 
 lemma build_forest'_simps[simp]:
-  "e = bs!k!i \<Longrightarrow> pointer e = Null \<Longrightarrow> build_trees' bs inp k i I = Some ([FBranch (item_rule_head (item e)) []])"
-  "e = bs!k!i \<Longrightarrow> pointer e = Pre pre \<Longrightarrow> build_trees' bs inp (k-1) pre {pre} = None \<Longrightarrow> build_trees' bs inp k i I = None"
-  "e = bs!k!i \<Longrightarrow> pointer e = Pre pre \<Longrightarrow> build_trees' bs inp (k-1) pre {pre} = Some pres \<Longrightarrow>
-    build_trees' bs inp k i I = those (map (\<lambda>f. case f of FBranch N fss \<Rightarrow> Some (FBranch N (fss @ [[FLeaf (inp!(k-1))]])) | _ \<Rightarrow> None) pres)"
+  "e = bs!k!i \<Longrightarrow> pointer e = Null \<Longrightarrow> build_trees' bs \<omega> k i I = Some ([FBranch (item_rule_head (item e)) []])"
+  "e = bs!k!i \<Longrightarrow> pointer e = Pre pre \<Longrightarrow> build_trees' bs \<omega> (k-1) pre {pre} = None \<Longrightarrow> build_trees' bs \<omega> k i I = None"
+  "e = bs!k!i \<Longrightarrow> pointer e = Pre pre \<Longrightarrow> build_trees' bs \<omega> (k-1) pre {pre} = Some pres \<Longrightarrow>
+    build_trees' bs \<omega> k i I = those (map (\<lambda>f. case f of FBranch N fss \<Rightarrow> Some (FBranch N (fss @ [[FLeaf (\<omega>!(k-1))]])) | _ \<Rightarrow> None) pres)"
   by (subst build_trees'.simps, simp)+
 
 definition wf_trees_input :: "('a bins \<times> 'a sentence \<times> nat \<times> nat \<times> nat set) set" where
   "wf_trees_input = {
-    (bs, inp, k, i, I) | bs inp k i I.
-      sound_ptrs inp bs \<and>
+    (bs, \<omega>, k, i, I) | bs \<omega> k i I.
+      sound_ptrs \<omega> bs \<and>
       k < length bs \<and>
       i < length (bs!k) \<and>
       I \<subseteq> {0..<length (bs!k)} \<and>
@@ -1587,24 +1595,24 @@ definition wf_trees_input :: "('a bins \<times> 'a sentence \<times> nat \<times
   }"
 
 fun build_forest'_measure :: "('a bins \<times> 'a sentence \<times> nat \<times> nat \<times> nat set) \<Rightarrow> nat" where
-  "build_forest'_measure (bs, inp, k, i, I) = foldl (+) 0 (map length (take (k+1) bs)) - card I"
+  "build_forest'_measure (bs, \<omega>, k, i, I) = foldl (+) 0 (map length (take (k+1) bs)) - card I"
 
 lemma wf_trees_input_pre:
-  assumes "(bs, inp, k, i, I) \<in> wf_trees_input"
+  assumes "(bs, \<omega>, k, i, I) \<in> wf_trees_input"
   assumes "e = bs!k!i" "pointer e = Pre pre"
-  shows "(bs, inp, (k-1), pre, {pre}) \<in> wf_trees_input"
+  shows "(bs, \<omega>, (k-1), pre, {pre}) \<in> wf_trees_input"
   using assms unfolding wf_trees_input_def
   apply (auto simp: sound_ptrs_def sound_pre_ptr_def)
   apply (metis nth_mem)
   done
 
 lemma wf_trees_input_prered_pre:
-  assumes "(bs, inp, k, i, I) \<in> wf_trees_input"
+  assumes "(bs, \<omega>, k, i, I) \<in> wf_trees_input"
   assumes "e = bs!k!i" "pointer e = PreRed p ps"
   assumes "ps' = filter (\<lambda>(k', pre, red). red \<notin> I) (p#ps)"
   assumes "gs = group_by (\<lambda>(k', pre, red). (k', pre)) (\<lambda>(k', pre, red). red) ps'"
   assumes "((k', pre), reds) \<in> set gs"
-  shows "(bs, inp, k', pre, {pre}) \<in> wf_trees_input"
+  shows "(bs, \<omega>, k', pre, {pre}) \<in> wf_trees_input"
 proof -
   obtain red where "(k', pre, red) \<in> set ps'"
     using assms(5,6) group_by_exists_kv by fast
@@ -1619,12 +1627,12 @@ proof -
 qed
 
 lemma wf_trees_input_prered_red:
-  assumes "(bs, inp, k, i, I) \<in> wf_trees_input"
+  assumes "(bs, \<omega>, k, i, I) \<in> wf_trees_input"
   assumes "e = bs!k!i" "pointer e = PreRed p ps"
   assumes "ps' = filter (\<lambda>(k', pre, red). red \<notin> I) (p#ps)"
   assumes "gs = group_by (\<lambda>(k', pre, red). (k', pre)) (\<lambda>(k', pre, red). red) ps'"
   assumes "((k', pre), reds) \<in> set gs" "red \<in> set reds"
-  shows "(bs, inp, k, red, I \<union> {red}) \<in> wf_trees_input"
+  shows "(bs, \<omega>, k, red, I \<union> {red}) \<in> wf_trees_input"
 proof -
   have "(k', pre, red) \<in> set ps'"
     using assms(5,6,7) group_by_forall_v_exists_k by fastforce
@@ -1643,21 +1651,21 @@ proof -
 qed
 
 lemma build_trees'_induct:
-  assumes "(bs, inp, k, i, I) \<in> wf_trees_input"
-  assumes "\<And>bs inp k i I.
-    (\<And>e pre. e = bs!k!i \<Longrightarrow> pointer e = Pre pre \<Longrightarrow> P bs inp (k-1) pre {pre}) \<Longrightarrow>
+  assumes "(bs, \<omega>, k, i, I) \<in> wf_trees_input"
+  assumes "\<And>bs \<omega> k i I.
+    (\<And>e pre. e = bs!k!i \<Longrightarrow> pointer e = Pre pre \<Longrightarrow> P bs \<omega> (k-1) pre {pre}) \<Longrightarrow>
     (\<And>e p ps ps' gs k' pre reds. e = bs!k!i \<Longrightarrow> pointer e = PreRed p ps \<Longrightarrow>
       ps' = filter (\<lambda>(k', pre, red). red \<notin> I) (p#ps) \<Longrightarrow>
       gs = group_by (\<lambda>(k', pre, red). (k', pre)) (\<lambda>(k', pre, red). red) ps' \<Longrightarrow>
-      ((k', pre), reds) \<in> set gs \<Longrightarrow> P bs inp k' pre {pre}) \<Longrightarrow>
+      ((k', pre), reds) \<in> set gs \<Longrightarrow> P bs \<omega> k' pre {pre}) \<Longrightarrow>
     (\<And>e p ps ps' gs k' pre red reds reds'. e = bs!k!i \<Longrightarrow> pointer e = PreRed p ps \<Longrightarrow>
       ps' = filter (\<lambda>(k', pre, red). red \<notin> I) (p#ps) \<Longrightarrow>
       gs = group_by (\<lambda>(k', pre, red). (k', pre)) (\<lambda>(k', pre, red). red) ps' \<Longrightarrow>
-      ((k', pre), reds) \<in> set gs \<Longrightarrow> red \<in> set reds \<Longrightarrow> P bs inp k red (I \<union> {red})) \<Longrightarrow>
-    P bs inp k i I" 
-  shows "P bs inp k i I"
+      ((k', pre), reds) \<in> set gs \<Longrightarrow> red \<in> set reds \<Longrightarrow> P bs \<omega> k red (I \<union> {red})) \<Longrightarrow>
+    P bs \<omega> k i I" 
+  shows "P bs \<omega> k i I"
   using assms(1)
-proof (induction n\<equiv>"build_forest'_measure (bs, inp, k, i, I)" arbitrary: k i I rule: nat_less_induct)
+proof (induction n\<equiv>"build_forest'_measure (bs, \<omega>, k, i, I)" arbitrary: k i I rule: nat_less_induct)
   case 1
   obtain e where entry: "e = bs!k!i"
     by simp
@@ -1674,7 +1682,7 @@ proof (induction n\<equiv>"build_forest'_measure (bs, inp, k, i, I)" arbitrary: 
     case Pre
     then obtain pre where pre: "pointer e = Pre pre"
       by blast
-    define n where n: "n = build_forest'_measure (bs, inp, (k-1), pre, {pre})"
+    define n where n: "n = build_forest'_measure (bs, \<omega>, (k-1), pre, {pre})"
     have "0 < k" "pre < length (bs!(k-1))"
       using 1(2) entry pre unfolding wf_trees_input_def sound_ptrs_def sound_pre_ptr_def
       by (smt (verit) mem_Collect_eq nth_mem prod.inject)+
@@ -1698,9 +1706,9 @@ proof (induction n\<equiv>"build_forest'_measure (bs, inp, k, i, I)" arbitrary: 
       by (simp add: \<open>card I \<le> length (bs ! k)\<close>)
     also have "... = foldl (+) 0 (map length (take (k+1) bs))"
       using foldl_add_nth \<open>k < length bs\<close> by blast
-    finally have "build_forest'_measure (bs, inp, k, i, I) - build_forest'_measure (bs, inp, (k-1), pre, {pre}) > 0"
+    finally have "build_forest'_measure (bs, \<omega>, k, i, I) - build_forest'_measure (bs, \<omega>, (k-1), pre, {pre}) > 0"
       by simp
-    hence "P bs inp (k-1) pre {pre}"
+    hence "P bs \<omega> (k-1) pre {pre}"
       using 1 n wf_trees_input_pre entry pre zero_less_diff by blast
     thus ?thesis
       using assms(2) entry pre pointer.distinct(5) pointer.inject(1) by presburger
@@ -1729,7 +1737,7 @@ proof (induction n\<equiv>"build_forest'_measure (bs, inp, k, i, I)" arbitrary: 
     {
       fix k' pre reds red
       assume a0: "((k', pre), reds) \<in> set gs"
-      define n_pre where n_pre: "n_pre = build_forest'_measure (bs, inp, k', pre, {pre})"
+      define n_pre where n_pre: "n_pre = build_forest'_measure (bs, \<omega>, k', pre, {pre})"
       have "k < length bs" "i < length (bs!k)" "I \<subseteq> {0..<length (bs!k)}" "i \<in> I"
         using 1(2) unfolding wf_trees_input_def by blast+
       have "k' < k" "pre < length (bs!k')"
@@ -1749,16 +1757,16 @@ proof (induction n\<equiv>"build_forest'_measure (bs, inp, k, i, I)" arbitrary: 
         using card_bound by simp
       also have "... \<le> foldl (+) 0 (map length (take (k+1) bs))"
         using foldl_add_nth_ge Suc_leI \<open>k < length bs\<close> \<open>k' < k\<close> by blast
-      finally have "build_forest'_measure (bs, inp, k, i, I) - build_forest'_measure (bs, inp, k', pre, {pre}) > 0"
+      finally have "build_forest'_measure (bs, \<omega>, k, i, I) - build_forest'_measure (bs, \<omega>, k', pre, {pre}) > 0"
         by simp
-      hence "P bs inp k' pre {pre}"
+      hence "P bs \<omega> k' pre {pre}"
         using 1(1) wf_trees_input_prered_pre[OF "1.prems"(1) entry pps ps' gs a0] zero_less_diff by blast
     }
     moreover {
       fix k' pre reds red
       assume a0: "((k', pre), reds) \<in> set gs"
       assume a1: "red \<in> set reds"
-      define n_red where n_red: "n_red = build_forest'_measure (bs, inp, k, red, I \<union> {red})"
+      define n_red where n_red: "n_red = build_forest'_measure (bs, \<omega>, k, red, I \<union> {red})"
       have "k < length bs" "i < length (bs!k)" "I \<subseteq> {0..<length (bs!k)}" "i \<in> I"
         using 1(2) unfolding wf_trees_input_def by blast+
       have "k' < k" "pre < length (bs!k')" "red < length (bs!k)"
@@ -1781,14 +1789,14 @@ proof (induction n\<equiv>"build_forest'_measure (bs, inp, k, i, I)" arbitrary: 
         using gt0 card_bound lt by force
       also have "... < foldl (+) 0 (map length (take (Suc k) bs))"
         using gt0 lt by auto
-      finally have "build_forest'_measure (bs, inp, k, i, I) - build_forest'_measure (bs, inp, k, red, I \<union> {red}) > 0"
+      finally have "build_forest'_measure (bs, \<omega>, k, i, I) - build_forest'_measure (bs, \<omega>, k, red, I \<union> {red}) > 0"
         by simp
-      moreover have "(bs, inp, k, red, I \<union> {red}) \<in> wf_trees_input"
+      moreover have "(bs, \<omega>, k, red, I \<union> {red}) \<in> wf_trees_input"
         using wf_trees_input_prered_red[OF "1"(2) entry pps ps' gs] a0 a1 by blast
-      ultimately have "P bs inp k red (I \<union> {red})"
+      ultimately have "P bs \<omega> k red (I \<union> {red})"
         using 1(1) zero_less_diff by blast
     }
-    moreover have "(\<And>e pre. e = bs!k!i \<Longrightarrow> pointer e = Pre pre \<Longrightarrow> P bs inp (k-1) pre {pre})"
+    moreover have "(\<And>e pre. e = bs!k!i \<Longrightarrow> pointer e = Pre pre \<Longrightarrow> P bs \<omega> (k-1) pre {pre})"
       using entry pps by fastforce
     ultimately show ?thesis
       using assms(2) entry gs pointer.inject(2) pps ps' by presburger
@@ -1796,12 +1804,12 @@ proof (induction n\<equiv>"build_forest'_measure (bs, inp, k, i, I)" arbitrary: 
 qed
 
 lemma build_trees'_termination:
-  assumes "(bs, inp, k, i, I) \<in> wf_trees_input"
-  shows "\<exists>fs. build_trees' bs inp k i I = Some fs \<and> (\<forall>f \<in> set fs. \<exists>N fss. f = FBranch N fss)"
+  assumes "(bs, \<omega>, k, i, I) \<in> wf_trees_input"
+  shows "\<exists>fs. build_trees' bs \<omega> k i I = Some fs \<and> (\<forall>f \<in> set fs. \<exists>N fss. f = FBranch N fss)"
 proof -
-  have "\<exists>fs. build_trees' bs inp k i I = Some fs \<and> (\<forall>f \<in> set fs. \<exists>N fss. f = FBranch N fss)"
+  have "\<exists>fs. build_trees' bs \<omega> k i I = Some fs \<and> (\<forall>f \<in> set fs. \<exists>N fss. f = FBranch N fss)"
     apply (induction rule: build_trees'_induct[OF assms(1)])
-    subgoal premises IH for bs inp k i I
+    subgoal premises IH for bs \<omega> k i I
     proof -
       define e where entry: "e = bs!k!i"
       consider (Null) "pointer e = Null"
@@ -1811,7 +1819,7 @@ proof -
       thus ?thesis
       proof cases
         case Null
-        have "build_trees' bs inp k i I = Some ([FBranch (item_rule_head (item e)) []])"
+        have "build_trees' bs \<omega> k i I = Some ([FBranch (item_rule_head (item e)) []])"
           using build_forest'_simps(1) Null entry by simp
         thus ?thesis
           by simp
@@ -1819,16 +1827,16 @@ proof -
         case Pre
         then obtain pre where pre: "pointer e = Pre pre"
           by blast
-        obtain fs where fs: "build_trees' bs inp (k-1) pre {pre} = Some fs"
+        obtain fs where fs: "build_trees' bs \<omega> (k-1) pre {pre} = Some fs"
           "\<forall>f \<in> set fs. \<exists>N fss. f = FBranch N fss"
           using IH(1) entry pre by blast
         let ?g = "\<lambda>f. case f of FLeaf a \<Rightarrow> None
-          | FBranch N fss \<Rightarrow> Some (FBranch N (fss @ [[FLeaf (inp!(k-1))]]))"
-        have simp: "build_trees' bs inp k i I = those (map ?g fs)"
+          | FBranch N fss \<Rightarrow> Some (FBranch N (fss @ [[FLeaf (\<omega>!(k-1))]]))"
+        have simp: "build_trees' bs \<omega> k i I = those (map ?g fs)"
           using build_forest'_simps(3) entry pre fs by blast
         moreover have "\<forall>f \<in> set (map ?g fs). \<exists>a. f = Some a"
           using fs(2) by auto
-        ultimately obtain fs' where fs': "build_trees' bs inp k i I = Some fs'"
+        ultimately obtain fs' where fs': "build_trees' bs \<omega> k i I = Some fs'"
           using those_Some by (smt (verit, best))
         moreover have "\<forall>f \<in> set fs'. \<exists>N fss. f = FBranch N fss"
         proof standard
@@ -1849,15 +1857,15 @@ proof -
         define gs where gs: "gs = group_by (\<lambda>(k', pre, red). (k', pre)) (\<lambda>(k', pre, red). red) ps'"
         let ?g = "\<lambda>((k', pre), reds).
             do {
-              pres \<leftarrow> build_trees' bs inp k' pre {pre};
-              rss \<leftarrow> those (map (\<lambda>red. build_trees' bs inp k red (I \<union> {red})) reds);
+              pres \<leftarrow> build_trees' bs \<omega> k' pre {pre};
+              rss \<leftarrow> those (map (\<lambda>red. build_trees' bs \<omega> k red (I \<union> {red})) reds);
               those (map (\<lambda>f.
                 case f of
                   FBranch N fss \<Rightarrow> Some (FBranch N (fss @ [concat rss]))
                 | _ \<Rightarrow> None \<comment>\<open>impossible case\<close>
               ) pres)
             }"
-        have simp: "build_trees' bs inp k i I = map_option concat (those (map ?g gs))"
+        have simp: "build_trees' bs \<omega> k i I = map_option concat (those (map ?g gs))"
           using entry pps ps' gs by (subst build_trees'.simps) (auto simp del: filter.simps)
         have "\<forall>fso \<in> set (map ?g gs). \<exists>fs. fso = Some fs \<and> (\<forall>f \<in> set fs. \<exists>N fss. f = FBranch N fss)"
         proof standard
@@ -1869,12 +1877,12 @@ proof -
             assume "ps \<in> set gs"
             then obtain k' pre reds where *: "((k', pre), reds) \<in> set gs" "((k', pre), reds) = ps"
               by (metis surj_pair)
-            then obtain pres where pres: "build_trees' bs inp k' pre {pre} = Some pres"
+            then obtain pres where pres: "build_trees' bs \<omega> k' pre {pre} = Some pres"
               "\<forall>f \<in> set pres. \<exists>N fss. f = FBranch N fss"
               using IH(2) entry pps ps' gs by blast
-            have "\<forall>f \<in> set (map (\<lambda>red. build_trees' bs inp k red (I \<union> {red})) reds). \<exists>a. f = Some a"
+            have "\<forall>f \<in> set (map (\<lambda>red. build_trees' bs \<omega> k red (I \<union> {red})) reds). \<exists>a. f = Some a"
               using IH(3)[OF entry pps ps' gs *(1)] by auto
-            then obtain rss where rss: "Some rss = those (map (\<lambda>red. build_trees' bs inp k red (I \<union> {red})) reds)"
+            then obtain rss where rss: "Some rss = those (map (\<lambda>red. build_trees' bs \<omega> k red (I \<union> {red})) reds)"
               using those_Some by (metis (full_types))
             let ?h = "\<lambda>f. case f of FBranch N fss \<Rightarrow> Some (FBranch N (fss @ [concat rss])) | _ \<Rightarrow> None"
             have "\<forall>x \<in> set (map ?h pres). \<exists>a. x = Some a"
@@ -1902,7 +1910,7 @@ proof -
         qed
         then obtain fss where "those (map ?g gs) = Some fss" "\<forall>fs \<in> set fss. \<forall>f \<in> set fs. \<exists>N fss. f = FBranch N fss"
           using those_Some_P by blast
-        hence "build_trees' bs inp k i I = Some (concat fss)" "\<forall>f \<in> set (concat fss). \<exists>N fss. f = FBranch N fss"
+        hence "build_trees' bs \<omega> k i I = Some (concat fss)" "\<forall>f \<in> set (concat fss). \<exists>N fss. f = FBranch N fss"
           using simp by auto
         thus ?thesis
           by blast
@@ -1914,18 +1922,18 @@ proof -
 qed
 
 lemma wf_item_tree_build_trees':
-  assumes "(bs, inp, k, i, I) \<in> wf_trees_input"
-  assumes "wf_bins cfg inp bs"
+  assumes "(bs, \<omega>, k, i, I) \<in> wf_trees_input"
+  assumes "wf_bins \<G> \<omega> bs"
   assumes "k < length bs" "i < length (bs!k)"
-  assumes "build_trees' bs inp k i I = Some fs"
+  assumes "build_trees' bs \<omega> k i I = Some fs"
   assumes "f \<in> set fs"
   assumes "t \<in> set (trees f)"
-  shows "wf_item_tree cfg (item (bs!k!i)) t"
+  shows "wf_item_tree \<G> (item (bs!k!i)) t"
 proof -
-  have "wf_item_tree cfg (item (bs!k!i)) t"
+  have "wf_item_tree \<G> (item (bs!k!i)) t"
     using assms
     apply (induction arbitrary: fs f t rule: build_trees'_induct[OF assms(1)])
-    subgoal premises prems for bs inp k i I fs f t
+    subgoal premises prems for bs \<omega> k i I fs f t
     proof -
       define e where entry: "e = bs!k!i"
       consider (Null) "pointer e = Null"
@@ -1935,13 +1943,13 @@ proof -
       thus ?thesis
       proof cases
         case Null
-        hence simp: "build_trees' bs inp k i I = Some ([FBranch (item_rule_head (item e)) []])"
+        hence simp: "build_trees' bs \<omega> k i I = Some ([FBranch (item_rule_head (item e)) []])"
           using entry by simp
         moreover have "f = FBranch (item_rule_head (item e)) []"
           using build_forest'_simps(1) Null prems(8,9) entry by auto
         ultimately have simp: "t = Branch (item_rule_head (item e)) []"
           using prems(10) by simp
-        have "sound_ptrs inp bs"
+        have "sound_ptrs \<omega> bs"
           using prems(4) unfolding wf_trees_input_def by blast
         hence "predicts (item e)"
           using Null prems(6,7) nth_mem entry unfolding sound_ptrs_def sound_null_ptr_def by blast
@@ -1953,38 +1961,38 @@ proof -
         case Pre
         then obtain pre where pre: "pointer e = Pre pre"
           by blast
-        have sound: "sound_ptrs inp bs"
+        have sound: "sound_ptrs \<omega> bs"
           using prems(4) unfolding wf_trees_input_def by blast
-        have scans: "scans inp k (item (bs!(k-1)!pre)) (item e)"
-          using entry pre prems(6-7) \<open>sound_ptrs inp bs\<close> unfolding sound_ptrs_def sound_pre_ptr_def by simp
+        have scans: "scans \<omega> k (item (bs!(k-1)!pre)) (item e)"
+          using entry pre prems(6-7) \<open>sound_ptrs \<omega> bs\<close> unfolding sound_ptrs_def sound_pre_ptr_def by simp
         hence *: 
           "item_rule_head (item (bs!(k-1)!pre)) = item_rule_head (item e)"
           "item_rule_body (item (bs!(k-1)!pre)) = item_rule_body (item e)"
           "item_dot (item (bs!(k-1)!pre)) + 1 = item_dot (item e)"
-          "next_symbol (item (bs!(k-1)!pre)) = Some (inp!(k-1))"
+          "next_symbol (item (bs!(k-1)!pre)) = Some (\<omega>!(k-1))"
           unfolding scans_def inc_item_def by (simp_all add: item_rule_head_def item_rule_body_def)
-        have wf: "(bs, inp, k-1, pre, {pre}) \<in> wf_trees_input"
+        have wf: "(bs, \<omega>, k-1, pre, {pre}) \<in> wf_trees_input"
           using entry pre prems(4) wf_trees_input_pre by blast
-        then obtain pres where pres: "build_trees' bs inp (k-1) pre {pre} = Some pres"
+        then obtain pres where pres: "build_trees' bs \<omega> (k-1) pre {pre} = Some pres"
           "\<forall>f \<in> set pres. \<exists>N fss. f = FBranch N fss"
           using build_trees'_termination wf by blast
-        let ?g = "\<lambda>f. case f of FBranch N fss \<Rightarrow> Some (FBranch N (fss @ [[FLeaf (inp!(k-1))]])) | _ \<Rightarrow> None"
-        have "build_trees' bs inp k i I = those (map ?g pres)"
+        let ?g = "\<lambda>f. case f of FBranch N fss \<Rightarrow> Some (FBranch N (fss @ [[FLeaf (\<omega>!(k-1))]])) | _ \<Rightarrow> None"
+        have "build_trees' bs \<omega> k i I = those (map ?g pres)"
           using entry pre pres by simp
         hence fs: "Some fs = those (map ?g pres)"
           using prems(8) by simp
-        then obtain f_pre N fss where Nfss: "f = FBranch N (fss @ [[FLeaf (inp!(k-1))]])"
+        then obtain f_pre N fss where Nfss: "f = FBranch N (fss @ [[FLeaf (\<omega>!(k-1))]])"
           "f_pre = FBranch N fss" "f_pre \<in> set pres"
           using those_map_FBranch_only fs pres(2) prems(9) by blast
         define tss where tss: "tss = map (\<lambda>fs. concat (map (\<lambda>f. trees f) fs)) fss"
-        have "trees (FBranch N (fss @ [[FLeaf (inp!(k-1))]])) = 
-          map (\<lambda>ts. Branch N ts) [ ts @ [Leaf (inp!(k-1))] . ts <- combinations tss ]"
+        have "trees (FBranch N (fss @ [[FLeaf (\<omega>!(k-1))]])) = 
+          map (\<lambda>ts. Branch N ts) [ ts @ [Leaf (\<omega>!(k-1))] . ts <- combinations tss ]"
           by (subst tss, subst trees_append_single_singleton, simp)
-        moreover have "t \<in> set (trees (FBranch N (fss @ [[FLeaf (inp!(k-1))]])))"
+        moreover have "t \<in> set (trees (FBranch N (fss @ [[FLeaf (\<omega>!(k-1))]])))"
           using Nfss(1) prems(10) by blast
-        ultimately obtain ts where ts: "t = Branch N (ts @ [Leaf (inp!(k-1))]) \<and> ts \<in> set (combinations tss)"
+        ultimately obtain ts where ts: "t = Branch N (ts @ [Leaf (\<omega>!(k-1))]) \<and> ts \<in> set (combinations tss)"
           by auto
-        have "sound_ptrs inp bs"
+        have "sound_ptrs \<omega> bs"
           using prems(4) unfolding wf_trees_input_def by blast
         hence "pre < length (bs!(k-1))"
           using entry pre prems(6,7) unfolding sound_ptrs_def sound_pre_ptr_def by (metis nth_mem)
@@ -1992,18 +2000,18 @@ proof -
           by (simp add: prems(6) less_imp_diff_less)
         moreover have "Branch N ts \<in> set (trees (FBranch N fss))"
           using ts tss by simp
-        ultimately have IH: "wf_item_tree cfg (item (bs!(k-1)!pre)) (Branch N ts)"
+        ultimately have IH: "wf_item_tree \<G> (item (bs!(k-1)!pre)) (Branch N ts)"
           using prems(1,2,4,5) entry pre Nfss(2,3) wf pres(1) by blast
-        have "map root_tree (ts @ [Leaf (inp!(k-1))]) = map root_tree ts @ [inp!(k-1)]"
+        have "map root_tree (ts @ [Leaf (\<omega>!(k-1))]) = map root_tree ts @ [\<omega>!(k-1)]"
           by simp
-        also have "... = take (item_dot (item (bs!(k-1)!pre))) (item_rule_body (item (bs!(k-1)!pre))) @ [inp!(k-1)]"
+        also have "... = take (item_dot (item (bs!(k-1)!pre))) (item_rule_body (item (bs!(k-1)!pre))) @ [\<omega>!(k-1)]"
           using IH by simp
-        also have "... = take (item_dot (item (bs!(k-1)!pre))) (item_rule_body (item e)) @ [inp!(k-1)]"
+        also have "... = take (item_dot (item (bs!(k-1)!pre))) (item_rule_body (item e)) @ [\<omega>!(k-1)]"
           using *(2) by simp
         also have "... = take (item_dot (item e)) (item_rule_body (item e))"
           using *(2-4) by (auto simp: next_symbol_def is_complete_def split: if_splits; metis leI take_Suc_conv_app_nth)
-        finally have "map root_tree (ts @ [Leaf (inp!(k-1))]) = take (item_dot (item e)) (item_rule_body (item e))" .
-        hence "wf_item_tree cfg (item e) (Branch N (ts @ [Leaf (inp!(k-1))]))"
+        finally have "map root_tree (ts @ [Leaf (\<omega>!(k-1))]) = take (item_dot (item e)) (item_rule_body (item e))" .
+        hence "wf_item_tree \<G> (item e) (Branch N (ts @ [Leaf (\<omega>!(k-1))]))"
           using IH *(1) by simp
         thus ?thesis
           using ts entry by fastforce
@@ -2015,43 +2023,43 @@ proof -
         define gs where gs: "gs = group_by (\<lambda>(k', pre, red). (k', pre)) (\<lambda>(k', pre, red). red) ps'"
         let ?g = "\<lambda>((k', pre), reds).
             do {
-              pres \<leftarrow> build_trees' bs inp k' pre {pre};
-              rss \<leftarrow> those (map (\<lambda>red. build_trees' bs inp k red (I \<union> {red})) reds);
+              pres \<leftarrow> build_trees' bs \<omega> k' pre {pre};
+              rss \<leftarrow> those (map (\<lambda>red. build_trees' bs \<omega> k red (I \<union> {red})) reds);
               those (map (\<lambda>f.
                 case f of
                   FBranch N fss \<Rightarrow> Some (FBranch N (fss @ [concat rss]))
                 | _ \<Rightarrow> None \<comment>\<open>impossible case\<close>
               ) pres)
             }"
-        have simp: "build_trees' bs inp k i I = map_option concat (those (map ?g gs))"
+        have simp: "build_trees' bs \<omega> k i I = map_option concat (those (map ?g gs))"
           using entry prered ps' gs by (subst build_trees'.simps) (auto simp del: filter.simps)
-        have "\<forall>fso \<in> set (map ?g gs). \<exists>fs. fso = Some fs \<and> (\<forall>f \<in> set fs. \<forall>t \<in> set (trees f). wf_item_tree cfg (item (bs!k!i)) t)"
+        have "\<forall>fso \<in> set (map ?g gs). \<exists>fs. fso = Some fs \<and> (\<forall>f \<in> set fs. \<forall>t \<in> set (trees f). wf_item_tree \<G> (item (bs!k!i)) t)"
         proof standard
           fix fso
           assume "fso \<in> set (map ?g gs)"
-          moreover have "\<forall>ps \<in> set gs. \<exists>fs. ?g ps = Some fs \<and> (\<forall>f \<in> set fs. \<forall>t \<in> set (trees f). wf_item_tree cfg (item (bs!k!i)) t)"
+          moreover have "\<forall>ps \<in> set gs. \<exists>fs. ?g ps = Some fs \<and> (\<forall>f \<in> set fs. \<forall>t \<in> set (trees f). wf_item_tree \<G> (item (bs!k!i)) t)"
           proof standard
             fix g
             assume "g \<in> set gs"
             then obtain k' pre reds where g: "((k', pre), reds) \<in> set gs" "((k', pre), reds) = g"
               by (metis surj_pair)
-            moreover have wf_pre: "(bs, inp, k', pre, {pre}) \<in> wf_trees_input"
+            moreover have wf_pre: "(bs, \<omega>, k', pre, {pre}) \<in> wf_trees_input"
               using wf_trees_input_prered_pre[OF prems(4) entry prered ps' gs g(1)] by blast
-            ultimately obtain pres where pres: "build_trees' bs inp k' pre {pre} = Some pres"
+            ultimately obtain pres where pres: "build_trees' bs \<omega> k' pre {pre} = Some pres"
               "\<forall>f_pre \<in> set pres. \<exists>N fss. f_pre = FBranch N fss"
               using build_trees'_termination by blast
-            have wf_reds: "\<forall>red \<in> set reds. (bs, inp, k, red, I \<union> {red}) \<in> wf_trees_input"
+            have wf_reds: "\<forall>red \<in> set reds. (bs, \<omega>, k, red, I \<union> {red}) \<in> wf_trees_input"
               using wf_trees_input_prered_red[OF prems(4) entry prered ps' gs g(1)] by blast
-            hence "\<forall>f \<in> set (map (\<lambda>red. build_trees' bs inp k red (I \<union> {red})) reds). \<exists>a. f = Some a"
+            hence "\<forall>f \<in> set (map (\<lambda>red. build_trees' bs \<omega> k red (I \<union> {red})) reds). \<exists>a. f = Some a"
               using build_trees'_termination by fastforce
-            then obtain rss where rss: "Some rss = those (map (\<lambda>red. build_trees' bs inp k red (I \<union> {red})) reds)"
+            then obtain rss where rss: "Some rss = those (map (\<lambda>red. build_trees' bs \<omega> k red (I \<union> {red})) reds)"
               using those_Some by (metis (full_types))
             let ?h = "\<lambda>f. case f of FBranch N fss \<Rightarrow> Some (FBranch N (fss @ [concat rss])) | _ \<Rightarrow> None"
             have "\<forall>x \<in> set (map ?h pres). \<exists>a. x = Some a"
               using pres(2) by auto
             then obtain fs where fs: "Some fs = those (map ?h pres)"
               using those_Some by (smt (verit, best))
-            have "\<forall>f \<in> set fs. \<forall>t \<in> set (trees f). wf_item_tree cfg (item (bs!k!i)) t"
+            have "\<forall>f \<in> set fs. \<forall>t \<in> set (trees f). wf_item_tree \<G> (item (bs!k!i)) t"
             proof (standard, standard)
               fix f t
               assume ft: "f \<in> set fs" "t \<in> set (trees f)"
@@ -2072,7 +2080,7 @@ proof -
                 by fastforce
               then obtain f_red where f_red: "f_red \<in> set (concat rss)" "ts1 \<in> set (trees f_red)"
                 by auto
-              obtain fs_red red where red: "Some fs_red = build_trees' bs inp k red (I \<union> {red})"
+              obtain fs_red red where red: "Some fs_red = build_trees' bs \<omega> k red (I \<union> {red})"
                 "f_red \<in> set fs_red" "red \<in> set reds"
                 using f_red(1) rss those_map_Some_concat_exists by fast
               then obtain N_red fss_red where "f_red = FBranch N_red fss_red"
@@ -2083,13 +2091,13 @@ proof -
                 using group_by_forall_v_exists_k \<open>((k', pre), reds) \<in> set gs\<close> gs \<open>red \<in> set reds\<close> by fast
               hence mem: "(k', pre, red) \<in> set (p#ps)"
                 using ps' by (metis filter_set member_filter)
-              have "sound_ptrs inp bs"
+              have "sound_ptrs \<omega> bs"
                 using prems(4) wf_trees_input_def by fastforce
               have bounds: "k' < k" "pre < length (bs!k')" "red < length (bs!k)"
-                using prered entry prems(6,7) \<open>sound_ptrs inp bs\<close>
+                using prered entry prems(6,7) \<open>sound_ptrs \<omega> bs\<close>
                 unfolding sound_ptrs_def sound_prered_ptr_def by (meson mem nth_mem)+
               have completes: "completes k (item (bs!k'!pre)) (item e) (item (bs!k!red))"
-                using prered entry prems(6,7) \<open>sound_ptrs inp bs\<close>
+                using prered entry prems(6,7) \<open>sound_ptrs \<omega> bs\<close>
                 unfolding sound_ptrs_def sound_prered_ptr_def by (metis mem nth_mem)
               have transform: 
                 "item_rule_head (item (bs!k'!pre)) = item_rule_head (item e)"
@@ -2101,10 +2109,10 @@ proof -
                 by (auto simp: item_rule_head_def item_rule_body_def is_complete_def)
               have "Branch N ts0 \<in> set (trees (FBranch N fss))"
                 using tss tsx(2) by simp
-              hence IH_pre: "wf_item_tree cfg (item (bs!k'!pre)) (Branch N ts0)"
+              hence IH_pre: "wf_item_tree \<G> (item (bs!k'!pre)) (Branch N ts0)"
                 using prems(2)[OF entry prered ps' gs \<open>((k', pre), reds) \<in> set gs\<close> wf_pre prems(5)]
                   pres(1) f_pre f_pre(3) bounds(1,2) prems(6) by fastforce
-              have IH_r: "wf_item_tree cfg (item (bs!k!red)) (Branch N_red ts)"
+              have IH_r: "wf_item_tree \<G> (item (bs!k!red)) (Branch N_red ts)"
                 using prems(3)[OF entry prered ps' gs \<open>((k', pre), reds) \<in> set gs\<close> \<open>red \<in> set reds\<close> _ prems(5)]
                   bounds(3) f_red(2) red ts wf_reds prems(6) by metis
               have "map root_tree (ts0 @ [Branch N_red ts]) = map root_tree ts0 @ [root_tree (Branch N_red ts)]"
@@ -2116,32 +2124,32 @@ proof -
               also have "... = take (item_dot (item e)) (item_rule_body (item e))"
                 using transform by (auto simp: next_symbol_def is_complete_def split: if_splits; metis leI take_Suc_conv_app_nth)
               finally have roots: "map root_tree (ts0 @ [Branch N_red ts]) = take (item_dot (item e)) (item_rule_body (item e))" .
-              have "wf_item cfg inp (item (bs!k!red))"
+              have "wf_item \<G> \<omega> (item (bs!k!red))"
                 using prems(5,6) bounds(3) unfolding wf_bins_def wf_bin_def wf_bin_items_def by (auto simp: items_def) 
               moreover have "N_red = item_rule_head (item (bs!k!red))"
                 using IH_r by fastforce
               moreover have "map root_tree ts = item_rule_body (item (bs!k!red))"
                 using IH_r transform(5) by (auto simp: is_complete_def)
-              ultimately have "\<exists>r \<in> set (\<RR> cfg). N_red = rule_head r \<and> map root_tree ts = rule_body r"
+              ultimately have "\<exists>r \<in> set (\<RR> \<G>). N_red = rule_head r \<and> map root_tree ts = rule_body r"
                 unfolding wf_item_def item_rule_body_def item_rule_head_def by blast
-              hence "wf_rule_tree cfg (Branch N_red ts)"
+              hence "wf_rule_tree \<G> (Branch N_red ts)"
                 using IH_r by simp
-              hence "wf_item_tree cfg (item (bs!k!i)) (Branch N (ts0 @ [Branch N_red ts]))"
+              hence "wf_item_tree \<G> (item (bs!k!i)) (Branch N (ts0 @ [Branch N_red ts]))"
                 using transform(1) roots IH_pre entry by simp
-              thus "wf_item_tree cfg (item (bs!k!i)) t"
+              thus "wf_item_tree \<G> (item (bs!k!i)) t"
                 using tsx(1) red ts by blast
             qed
             moreover have "?g g = Some fs"
               using fs pres rss g by (auto, metis bind.bind_lunit)
-            ultimately show "\<exists>fs. ?g g = Some fs \<and> (\<forall>f \<in> set fs. \<forall>t \<in> set (trees f). wf_item_tree cfg (item (bs!k!i)) t)"
+            ultimately show "\<exists>fs. ?g g = Some fs \<and> (\<forall>f \<in> set fs. \<forall>t \<in> set (trees f). wf_item_tree \<G> (item (bs!k!i)) t)"
               by blast
           qed
-          ultimately show "\<exists>fs. fso = Some fs \<and> (\<forall>f \<in> set fs. \<forall>t \<in> set (trees f). wf_item_tree cfg (item (bs!k!i)) t)"
+          ultimately show "\<exists>fs. fso = Some fs \<and> (\<forall>f \<in> set fs. \<forall>t \<in> set (trees f). wf_item_tree \<G> (item (bs!k!i)) t)"
             using map_Some_P by auto
         qed
-        then obtain fss where "those (map ?g gs) = Some fss" "\<forall>fs \<in> set fss. \<forall>f \<in> set fs. \<forall>t \<in> set (trees f). wf_item_tree cfg (item (bs!k!i)) t"
+        then obtain fss where "those (map ?g gs) = Some fss" "\<forall>fs \<in> set fss. \<forall>f \<in> set fs. \<forall>t \<in> set (trees f). wf_item_tree \<G> (item (bs!k!i)) t"
           using those_Some_P by blast
-        hence "build_trees' bs inp k i I = Some (concat fss)" "\<forall>f \<in> set (concat fss). \<forall>t \<in> set (trees f). wf_item_tree cfg (item (bs!k!i)) t"
+        hence "build_trees' bs \<omega> k i I = Some (concat fss)" "\<forall>f \<in> set (concat fss). \<forall>t \<in> set (trees f). wf_item_tree \<G> (item (bs!k!i)) t"
           using simp by auto
         thus ?thesis
           using prems(8-10) by auto
@@ -2153,18 +2161,18 @@ proof -
 qed
 
 lemma wf_yield_tree_build_trees':
-  assumes "(bs, inp, k, i, I) \<in> wf_trees_input"
-  assumes "wf_bins cfg inp bs"
-  assumes "k < length bs" "i < length (bs!k)" "k \<le> length inp"
-  assumes "build_trees' bs inp k i I = Some fs"
+  assumes "(bs, \<omega>, k, i, I) \<in> wf_trees_input"
+  assumes "wf_bins \<G> \<omega> bs"
+  assumes "k < length bs" "i < length (bs!k)" "k \<le> length \<omega>"
+  assumes "build_trees' bs \<omega> k i I = Some fs"
   assumes "f \<in> set fs"
   assumes "t \<in> set (trees f)"
-  shows "wf_yield_tree inp (item (bs!k!i)) t"
+  shows "wf_yield_tree \<omega> (item (bs!k!i)) t"
 proof -
-  have "wf_yield_tree inp (item (bs!k!i)) t"
+  have "wf_yield_tree \<omega> (item (bs!k!i)) t"
     using assms
     apply (induction arbitrary: fs f t rule: build_trees'_induct[OF assms(1)])
-    subgoal premises prems for bs inp k i I fs f t
+    subgoal premises prems for bs \<omega> k i I fs f t
     proof -
       define e where entry: "e = bs!k!i"
       consider (Null) "pointer e = Null"
@@ -2174,13 +2182,13 @@ proof -
       thus ?thesis
       proof cases
         case Null
-        hence simp: "build_trees' bs inp k i I = Some ([FBranch (item_rule_head (item e)) []])"
+        hence simp: "build_trees' bs \<omega> k i I = Some ([FBranch (item_rule_head (item e)) []])"
           using entry by simp
         moreover have "f = FBranch (item_rule_head (item e)) []"
           using build_forest'_simps(1) Null prems(9,10) entry by auto
         ultimately have simp: "t = Branch (item_rule_head (item e)) []"
           using prems(11) by simp
-        have "sound_ptrs inp bs"
+        have "sound_ptrs \<omega> bs"
           using prems(4) unfolding wf_trees_input_def by blast
         hence "predicts (item e)"
           using Null prems(6,7) nth_mem entry unfolding sound_ptrs_def sound_null_ptr_def by blast
@@ -2190,34 +2198,34 @@ proof -
         case Pre
         then obtain pre where pre: "pointer e = Pre pre"
           by blast
-        have sound: "sound_ptrs inp bs"
+        have sound: "sound_ptrs \<omega> bs"
           using prems(4) unfolding wf_trees_input_def by blast
         hence bounds:  "k > 0" "pre < length (bs!(k-1))"
           using entry pre prems(6,7) unfolding sound_ptrs_def sound_pre_ptr_def by (metis nth_mem)+
-        have scans: "scans inp k (item (bs!(k-1)!pre)) (item e)"
-          using entry pre prems(6-7) \<open>sound_ptrs inp bs\<close> unfolding sound_ptrs_def sound_pre_ptr_def by simp
-        have wf: "(bs, inp, k-1, pre, {pre}) \<in> wf_trees_input"
+        have scans: "scans \<omega> k (item (bs!(k-1)!pre)) (item e)"
+          using entry pre prems(6-7) \<open>sound_ptrs \<omega> bs\<close> unfolding sound_ptrs_def sound_pre_ptr_def by simp
+        have wf: "(bs, \<omega>, k-1, pre, {pre}) \<in> wf_trees_input"
           using entry pre prems(4) wf_trees_input_pre by blast
-        then obtain pres where pres: "build_trees' bs inp (k-1) pre {pre} = Some pres"
+        then obtain pres where pres: "build_trees' bs \<omega> (k-1) pre {pre} = Some pres"
           "\<forall>f \<in> set pres. \<exists>N fss. f = FBranch N fss"
           using build_trees'_termination wf by blast
-        let ?g = "\<lambda>f. case f of FBranch N fss \<Rightarrow> Some (FBranch N (fss @ [[FLeaf (inp!(k-1))]])) | _ \<Rightarrow> None"
-        have "build_trees' bs inp k i I = those (map ?g pres)"
+        let ?g = "\<lambda>f. case f of FBranch N fss \<Rightarrow> Some (FBranch N (fss @ [[FLeaf (\<omega>!(k-1))]])) | _ \<Rightarrow> None"
+        have "build_trees' bs \<omega> k i I = those (map ?g pres)"
           using entry pre pres by simp
         hence fs: "Some fs = those (map ?g pres)"
           using prems(9) by simp
-        then obtain f_pre N fss where Nfss: "f = FBranch N (fss @ [[FLeaf (inp!(k-1))]])"
+        then obtain f_pre N fss where Nfss: "f = FBranch N (fss @ [[FLeaf (\<omega>!(k-1))]])"
           "f_pre = FBranch N fss" "f_pre \<in> set pres"
           using those_map_FBranch_only fs pres(2) prems(10) by blast
         define tss where tss: "tss = map (\<lambda>fs. concat (map (\<lambda>f. trees f) fs)) fss"
-        have "trees (FBranch N (fss @ [[FLeaf (inp!(k-1))]])) = 
-          map (\<lambda>ts. Branch N ts) [ ts @ [Leaf (inp!(k-1))] . ts <- combinations tss ]"
+        have "trees (FBranch N (fss @ [[FLeaf (\<omega>!(k-1))]])) = 
+          map (\<lambda>ts. Branch N ts) [ ts @ [Leaf (\<omega>!(k-1))] . ts <- combinations tss ]"
           by (subst tss, subst trees_append_single_singleton, simp)
-        moreover have "t \<in> set (trees (FBranch N (fss @ [[FLeaf (inp!(k-1))]])))"
+        moreover have "t \<in> set (trees (FBranch N (fss @ [[FLeaf (\<omega>!(k-1))]])))"
           using Nfss(1) prems(11) by blast
-        ultimately obtain ts where ts: "t = Branch N (ts @ [Leaf (inp!(k-1))]) \<and> ts \<in> set (combinations tss)"
+        ultimately obtain ts where ts: "t = Branch N (ts @ [Leaf (\<omega>!(k-1))]) \<and> ts \<in> set (combinations tss)"
           by auto
-        have "sound_ptrs inp bs"
+        have "sound_ptrs \<omega> bs"
           using prems(4) unfolding wf_trees_input_def by blast
         hence "pre < length (bs!(k-1))"
           using entry pre prems(6,7) unfolding sound_ptrs_def sound_pre_ptr_def by (metis nth_mem)
@@ -2225,7 +2233,7 @@ proof -
           by (simp add: prems(6) less_imp_diff_less)
         moreover have "Branch N ts \<in> set (trees (FBranch N fss))"
           using ts tss by simp
-        ultimately have IH: "wf_yield_tree inp (item (bs!(k-1)!pre)) (Branch N ts)"
+        ultimately have IH: "wf_yield_tree \<omega> (item (bs!(k-1)!pre)) (Branch N ts)"
           using prems(1,2,4,5,8) entry pre Nfss(2,3) wf pres(1) by simp
         have transform: 
           "item_origin (item (bs!(k-1)!pre)) \<le> item_end (item (bs!(k-1)!pre))"
@@ -2233,20 +2241,20 @@ proof -
           "item_end (item e) = k"
           using entry prems(5,6,7) bounds unfolding wf_bins_def wf_bin_def wf_bin_items_def items_def wf_item_def
           by (auto, meson less_imp_diff_less nth_mem)
-        have "yield_tree t = concat (map yield_tree (ts @ [Leaf (inp!(k-1))]))"
+        have "yield_tree t = concat (map yield_tree (ts @ [Leaf (\<omega>!(k-1))]))"
           by (simp add: ts)
-        also have "... = concat (map yield_tree ts) @ [inp!(k-1)]"
+        also have "... = concat (map yield_tree ts) @ [\<omega>!(k-1)]"
           by simp
-        also have "... = slice (item_origin (item (bs!(k-1)!pre))) (item_end (item (bs!(k-1)!pre))) inp @ [inp!(k-1)]"
+        also have "... = slice (item_origin (item (bs!(k-1)!pre))) (item_end (item (bs!(k-1)!pre))) \<omega> @ [\<omega>!(k-1)]"
           using IH by (simp add: wf_yield_tree_def)
-        also have "... = slice (item_origin (item (bs!(k-1)!pre))) (item_end (item (bs!(k-1)!pre)) + 1) inp"
+        also have "... = slice (item_origin (item (bs!(k-1)!pre))) (item_end (item (bs!(k-1)!pre)) + 1) \<omega>"
           using slice_append_nth transform \<open>k > 0\<close> prems(8)
           by (metis diff_less le_eq_less_or_eq less_imp_diff_less less_numeral_extra(1))
-        also have "... = slice (item_origin (item e)) (item_end (item (bs!(k-1)!pre)) + 1) inp"
+        also have "... = slice (item_origin (item e)) (item_end (item (bs!(k-1)!pre)) + 1) \<omega>"
           using scans unfolding scans_def inc_item_def by simp
-        also have "... = slice (item_origin (item e)) k inp"
+        also have "... = slice (item_origin (item e)) k \<omega>"
           using scans transform unfolding scans_def by (metis Suc_diff_1 Suc_eq_plus1 bounds(1))
-        also have "... = slice (item_origin (item e)) (item_end (item e)) inp"
+        also have "... = slice (item_origin (item e)) (item_end (item e)) \<omega>"
           using transform by auto
         finally show ?thesis
           using wf_yield_tree_def entry by blast
@@ -2258,43 +2266,43 @@ proof -
         define gs where gs: "gs = group_by (\<lambda>(k', pre, red). (k', pre)) (\<lambda>(k', pre, red). red) ps'"
         let ?g = "\<lambda>((k', pre), reds).
             do {
-              pres \<leftarrow> build_trees' bs inp k' pre {pre};
-              rss \<leftarrow> those (map (\<lambda>red. build_trees' bs inp k red (I \<union> {red})) reds);
+              pres \<leftarrow> build_trees' bs \<omega> k' pre {pre};
+              rss \<leftarrow> those (map (\<lambda>red. build_trees' bs \<omega> k red (I \<union> {red})) reds);
               those (map (\<lambda>f.
                 case f of
                   FBranch N fss \<Rightarrow> Some (FBranch N (fss @ [concat rss]))
                 | _ \<Rightarrow> None \<comment>\<open>impossible case\<close>
               ) pres)
             }"
-        have simp: "build_trees' bs inp k i I = map_option concat (those (map ?g gs))"
+        have simp: "build_trees' bs \<omega> k i I = map_option concat (those (map ?g gs))"
           using entry prered ps' gs by (subst build_trees'.simps) (auto simp del: filter.simps)
-        have "\<forall>fso \<in> set (map ?g gs). \<exists>fs. fso = Some fs \<and> (\<forall>f \<in> set fs. \<forall>t \<in> set (trees f). wf_yield_tree inp (item (bs!k!i)) t)"
+        have "\<forall>fso \<in> set (map ?g gs). \<exists>fs. fso = Some fs \<and> (\<forall>f \<in> set fs. \<forall>t \<in> set (trees f). wf_yield_tree \<omega> (item (bs!k!i)) t)"
         proof standard
           fix fso
           assume "fso \<in> set (map ?g gs)"
-          moreover have "\<forall>ps \<in> set gs. \<exists>fs. ?g ps = Some fs \<and> (\<forall>f \<in> set fs. \<forall>t \<in> set (trees f). wf_yield_tree inp (item (bs!k!i)) t)"
+          moreover have "\<forall>ps \<in> set gs. \<exists>fs. ?g ps = Some fs \<and> (\<forall>f \<in> set fs. \<forall>t \<in> set (trees f). wf_yield_tree \<omega> (item (bs!k!i)) t)"
           proof standard
             fix g
             assume "g \<in> set gs"
             then obtain k' pre reds where g: "((k', pre), reds) \<in> set gs" "((k', pre), reds) = g"
               by (metis surj_pair)
-            moreover have wf_pre: "(bs, inp, k', pre, {pre}) \<in> wf_trees_input"
+            moreover have wf_pre: "(bs, \<omega>, k', pre, {pre}) \<in> wf_trees_input"
               using wf_trees_input_prered_pre[OF prems(4) entry prered ps' gs g(1)] by blast
-            ultimately obtain pres where pres: "build_trees' bs inp k' pre {pre} = Some pres"
+            ultimately obtain pres where pres: "build_trees' bs \<omega> k' pre {pre} = Some pres"
               "\<forall>f_pre \<in> set pres. \<exists>N fss. f_pre = FBranch N fss"
               using build_trees'_termination by blast
-            have wf_reds: "\<forall>red \<in> set reds. (bs, inp, k, red, I \<union> {red}) \<in> wf_trees_input"
+            have wf_reds: "\<forall>red \<in> set reds. (bs, \<omega>, k, red, I \<union> {red}) \<in> wf_trees_input"
               using wf_trees_input_prered_red[OF prems(4) entry prered ps' gs g(1)] by blast
-            hence "\<forall>f \<in> set (map (\<lambda>red. build_trees' bs inp k red (I \<union> {red})) reds). \<exists>a. f = Some a"
+            hence "\<forall>f \<in> set (map (\<lambda>red. build_trees' bs \<omega> k red (I \<union> {red})) reds). \<exists>a. f = Some a"
               using build_trees'_termination by fastforce
-            then obtain rss where rss: "Some rss = those (map (\<lambda>red. build_trees' bs inp k red (I \<union> {red})) reds)"
+            then obtain rss where rss: "Some rss = those (map (\<lambda>red. build_trees' bs \<omega> k red (I \<union> {red})) reds)"
               using those_Some by (metis (full_types))
             let ?h = "\<lambda>f. case f of FBranch N fss \<Rightarrow> Some (FBranch N (fss @ [concat rss])) | _ \<Rightarrow> None"
             have "\<forall>x \<in> set (map ?h pres). \<exists>a. x = Some a"
               using pres(2) by auto
             then obtain fs where fs: "Some fs = those (map ?h pres)"
               using those_Some by (smt (verit, best))
-            have "\<forall>f \<in> set fs. \<forall>t \<in> set (trees f). wf_yield_tree inp (item (bs!k!i)) t"
+            have "\<forall>f \<in> set fs. \<forall>t \<in> set (trees f). wf_yield_tree \<omega> (item (bs!k!i)) t"
             proof (standard, standard)
               fix f t
               assume ft: "f \<in> set fs" "t \<in> set (trees f)"
@@ -2315,7 +2323,7 @@ proof -
                 by fastforce
               then obtain f_red where f_red: "f_red \<in> set (concat rss)" "ts1 \<in> set (trees f_red)"
                 by auto
-              obtain fs_red red where red: "Some fs_red = build_trees' bs inp k red (I \<union> {red})"
+              obtain fs_red red where red: "Some fs_red = build_trees' bs \<omega> k red (I \<union> {red})"
                 "f_red \<in> set fs_red" "red \<in> set reds"
                 using f_red(1) rss those_map_Some_concat_exists by fast
               then obtain N_red fss_red where "f_red = FBranch N_red fss_red"
@@ -2326,13 +2334,13 @@ proof -
                 using group_by_forall_v_exists_k \<open>((k', pre), reds) \<in> set gs\<close> gs \<open>red \<in> set reds\<close> by fast
               hence mem: "(k', pre, red) \<in> set (p#ps)"
                 using ps' by (metis filter_set member_filter)
-              have "sound_ptrs inp bs"
+              have "sound_ptrs \<omega> bs"
                 using prems(4) wf_trees_input_def by fastforce
               have bounds: "k' < k" "pre < length (bs!k')" "red < length (bs!k)"
-                using prered entry prems(6,7) \<open>sound_ptrs inp bs\<close>
+                using prered entry prems(6,7) \<open>sound_ptrs \<omega> bs\<close>
                 unfolding sound_ptrs_def sound_prered_ptr_def by (meson mem nth_mem)+
               have completes: "completes k (item (bs!k'!pre)) (item e) (item (bs!k!red))"
-                using prered entry prems(6,7) \<open>sound_ptrs inp bs\<close>
+                using prered entry prems(6,7) \<open>sound_ptrs \<omega> bs\<close>
                 unfolding sound_ptrs_def sound_prered_ptr_def by (metis mem nth_mem)
               have transform: 
                 "item_rule_head (item (bs!k'!pre)) = item_rule_head (item e)"
@@ -2344,10 +2352,10 @@ proof -
                 by (auto simp: item_rule_head_def item_rule_body_def is_complete_def)
               have "Branch N ts0 \<in> set (trees (FBranch N fss))"
                 using tss tsx(2) by simp
-              hence IH_pre: "wf_yield_tree inp (item (bs!k'!pre)) (Branch N ts0)"
+              hence IH_pre: "wf_yield_tree \<omega> (item (bs!k'!pre)) (Branch N ts0)"
                 using prems(2)[OF entry prered ps' gs \<open>((k', pre), reds) \<in> set gs\<close> wf_pre prems(5)]
                   pres(1) f_pre f_pre(3) bounds(1,2) prems(6,8) by simp
-              have IH_r: "wf_yield_tree inp (item (bs!k!red)) (Branch N_red ts)"
+              have IH_r: "wf_yield_tree \<omega> (item (bs!k!red)) (Branch N_red ts)"
                 using prems(3)[OF entry prered ps' gs \<open>((k', pre), reds) \<in> set gs\<close> \<open>red \<in> set reds\<close> _ prems(5)]
                   bounds(3) f_red(2) red ts wf_reds prems(6,8) by metis
               have wf1: 
@@ -2363,29 +2371,29 @@ proof -
                 by (simp add: ts tsx(1))
               also have "... = concat (map yield_tree ts0) @ yield_tree (Branch N_red ts)"
                 by simp
-              also have "... = slice (item_origin (item (bs!k'!pre))) (item_end (item (bs!k'!pre))) inp @ 
-                slice (item_origin (item (bs!k!red))) (item_end (item (bs!k!red))) inp"
+              also have "... = slice (item_origin (item (bs!k'!pre))) (item_end (item (bs!k'!pre))) \<omega> @ 
+                slice (item_origin (item (bs!k!red))) (item_end (item (bs!k!red))) \<omega>"
                 using IH_pre IH_r by (simp add: wf_yield_tree_def)
-              also have "... = slice (item_origin (item (bs!k'!pre))) (item_end (item (bs!k!red))) inp"
+              also have "... = slice (item_origin (item (bs!k'!pre))) (item_end (item (bs!k!red))) \<omega>"
                 using slice_concat wf1 completes_def completes by (metis (no_types, lifting))
-              also have "... = slice (item_origin (item e)) (item_end (item (bs!k!red))) inp"
+              also have "... = slice (item_origin (item e)) (item_end (item (bs!k!red))) \<omega>"
                 using completes unfolding completes_def inc_item_def by simp
-              also have "... = slice (item_origin (item e)) (item_end (item e)) inp"
+              also have "... = slice (item_origin (item e)) (item_end (item e)) \<omega>"
                 using wf2 entry by presburger
-              finally show "wf_yield_tree inp (item (bs!k!i)) t"
+              finally show "wf_yield_tree \<omega> (item (bs!k!i)) t"
                 using wf_yield_tree_def entry by blast
             qed
             moreover have "?g g = Some fs"
               using fs pres rss g by (auto, metis bind.bind_lunit)
-            ultimately show "\<exists>fs. ?g g = Some fs \<and> (\<forall>f \<in> set fs. \<forall>t \<in> set (trees f). wf_yield_tree inp (item (bs!k!i)) t)"
+            ultimately show "\<exists>fs. ?g g = Some fs \<and> (\<forall>f \<in> set fs. \<forall>t \<in> set (trees f). wf_yield_tree \<omega> (item (bs!k!i)) t)"
               by blast
           qed
-          ultimately show "\<exists>fs. fso = Some fs \<and> (\<forall>f \<in> set fs. \<forall>t \<in> set (trees f). wf_yield_tree inp (item (bs!k!i)) t)"
+          ultimately show "\<exists>fs. fso = Some fs \<and> (\<forall>f \<in> set fs. \<forall>t \<in> set (trees f). wf_yield_tree \<omega> (item (bs!k!i)) t)"
             using map_Some_P by auto
         qed
-        then obtain fss where "those (map ?g gs) = Some fss" "\<forall>fs \<in> set fss. \<forall>f \<in> set fs. \<forall>t \<in> set (trees f). wf_yield_tree inp (item (bs!k!i)) t"
+        then obtain fss where "those (map ?g gs) = Some fss" "\<forall>fs \<in> set fss. \<forall>f \<in> set fs. \<forall>t \<in> set (trees f). wf_yield_tree \<omega> (item (bs!k!i)) t"
           using those_Some_P by blast
-        hence "build_trees' bs inp k i I = Some (concat fss)" "\<forall>f \<in> set (concat fss). \<forall>t \<in> set (trees f). wf_yield_tree inp (item (bs!k!i)) t"
+        hence "build_trees' bs \<omega> k i I = Some (concat fss)" "\<forall>f \<in> set (concat fss). \<forall>t \<in> set (trees f). wf_yield_tree \<omega> (item (bs!k!i)) t"
           using simp by auto
         thus ?thesis
           using prems(9-11) by auto
@@ -2397,34 +2405,34 @@ proof -
 qed
 
 theorem wf_rule_root_yield_tree_build_trees:
-  assumes "wf_bins cfg inp bs" "sound_ptrs inp bs" "length bs = length inp + 1"
-  assumes "build_trees cfg inp bs = Some fs" "f \<in> set fs" "t \<in> set (trees f)"
-  shows "wf_rule_tree cfg t \<and> root_tree t = \<SS> cfg \<and> yield_tree t = inp"
+  assumes "wf_bins \<G> \<omega> bs" "sound_ptrs \<omega> bs" "length bs = length \<omega> + 1"
+  assumes "build_trees \<G> \<omega> bs = Some fs" "f \<in> set fs" "t \<in> set (trees f)"
+  shows "wf_rule_tree \<G> t \<and> root_tree t = \<SS> \<G> \<and> yield_tree t = \<omega>"
 proof -
   let ?k = "length bs - 1"
-  define finished where finished_def: "finished = filter_with_index (is_finished cfg inp) (items (bs!?k))"
-  have #: "Some fs = map_option concat (those (map (\<lambda>(_, i). build_trees' bs inp ?k i {i}) finished))"
+  define finished where finished_def: "finished = filter_with_index (is_finished \<G> \<omega>) (items (bs!?k))"
+  have #: "Some fs = map_option concat (those (map (\<lambda>(_, i). build_trees' bs \<omega> ?k i {i}) finished))"
     using assms(4) build_trees_def finished_def by (metis (full_types))
-  then obtain fss fs' where fss: "Some fss = those (map (\<lambda>(_, i). build_trees' bs inp ?k i {i}) finished)"
+  then obtain fss fs' where fss: "Some fss = those (map (\<lambda>(_, i). build_trees' bs \<omega> ?k i {i}) finished)"
     "fs' \<in> set fss" "f \<in> set fs'"
     using map_option_concat_those_map_exists assms(5) by fastforce
-  then obtain x i where *: "(x,i) \<in> set finished" "Some fs' =  build_trees' bs inp (length bs - 1) i {i}"
+  then obtain x i where *: "(x,i) \<in> set finished" "Some fs' =  build_trees' bs \<omega> (length bs - 1) i {i}"
     using those_map_exists[OF fss(1,2)] by auto
-  have k: "?k < length bs" "?k \<le> length inp"
+  have k: "?k < length bs" "?k \<le> length \<omega>"
     using assms(3) by simp_all
   have i: "i < length (bs!?k)"
     using index_filter_with_index_lt_length * items_def finished_def by (metis (no_types, opaque_lifting) length_map)
   have x: "x = item (bs!?k!i)"
     using * i filter_with_index_nth items_def nth_map finished_def assms(3) by metis
-  have finished: "is_finished cfg inp x"
+  have finished: "is_finished \<G> \<omega> x"
     using * filter_with_index_P finished_def by metis
   have "{i} \<subseteq> {0..<length (bs!?k)}"
     using atLeastLessThan_iff i by blast
-  hence wf: "(bs, inp, ?k, i, {i}) \<in> wf_trees_input"
+  hence wf: "(bs, \<omega>, ?k, i, {i}) \<in> wf_trees_input"
     unfolding wf_trees_input_def using assms(2) i k(1) by simp
-  hence wf_item_tree: "wf_item_tree cfg (item (bs!?k!i)) t"
+  hence wf_item_tree: "wf_item_tree \<G> (item (bs!?k!i)) t"
     using wf_item_tree_build_trees' assms(1,2,5,6) i k(1) x *(2) fss(3) by metis
-  have wf_item: "wf_item cfg inp (item (bs!?k!i))"
+  have wf_item: "wf_item \<G> \<omega> (item (bs!?k!i))"
     using k(1) i assms(1) unfolding wf_bins_def wf_bin_def wf_bin_items_def by (simp add: items_def)
   obtain N fss where Nfss: "f = FBranch N fss"
     using build_trees'_termination[OF wf] by (metis "*"(2) fss(3) option.inject)
@@ -2433,86 +2441,84 @@ proof -
   hence "N = item_rule_head x"
     "map root_tree ts = item_rule_body x"
     using finished wf_item_tree x by (auto simp: is_finished_def is_complete_def)
-  hence "\<exists>r \<in> set (\<RR> cfg). N = rule_head r \<and> map root_tree ts = rule_body r"
+  hence "\<exists>r \<in> set (\<RR> \<G>). N = rule_head r \<and> map root_tree ts = rule_body r"
     using wf_item x unfolding wf_item_def item_rule_body_def item_rule_head_def by blast
-  hence wf_rule: "wf_rule_tree cfg t"
+  hence wf_rule: "wf_rule_tree \<G> t"
     using wf_item_tree ts by simp
-  have root: "root_tree t = \<SS> cfg"
+  have root: "root_tree t = \<SS> \<G>"
     using finished ts \<open>N = item_rule_head x\<close> by (auto simp: is_finished_def)
-  have "yield_tree t = slice (item_origin (item (bs!?k!i))) (item_end (item (bs!?k!i))) inp"
+  have "yield_tree t = slice (item_origin (item (bs!?k!i))) (item_end (item (bs!?k!i))) \<omega>"
     using k i assms(1,6) wf wf_yield_tree_build_trees' wf_yield_tree_def *(2) fss(3) by (smt (verit, best))
-  hence yield: "yield_tree t = inp"
+  hence yield: "yield_tree t = \<omega>"
     using finished x unfolding is_finished_def by simp
   show ?thesis
     using * wf_rule root yield assms(4) unfolding build_trees_def by simp
 qed
 
 corollary wf_rule_root_yield_tree_build_trees_Earley\<^sub>L:
-  assumes "wf_\<G> cfg" "nonempty_derives cfg"
-  assumes "build_trees cfg inp (Earley\<^sub>L cfg inp) = Some fs" "f \<in> set fs" "t \<in> set (trees f)"
-  shows "wf_rule_tree cfg t \<and> root_tree t = \<SS> cfg \<and> yield_tree t = inp"
+  assumes "wf_\<G> \<G>" "nonempty_derives \<G>"
+  assumes "build_trees \<G> \<omega> (Earley\<^sub>L \<G> \<omega>) = Some fs" "f \<in> set fs" "t \<in> set (trees f)"
+  shows "wf_rule_tree \<G> t \<and> root_tree t = \<SS> \<G> \<and> yield_tree t = \<omega>"
   using assms wf_rule_root_yield_tree_build_trees wf_bins_Earley\<^sub>L Earley\<^sub>L_def
     length_Earley\<^sub>L_bins length_bins_Init\<^sub>L sound_mono_ptrs_Earley\<^sub>L
   by (metis dual_order.eq_iff )
 
 theorem soundness_build_trees_Earley\<^sub>L:
-  assumes "wf_\<G> cfg" "is_word cfg inp" "nonempty_derives cfg"
-  assumes "build_trees cfg inp (Earley\<^sub>L cfg inp) = Some fs" "f \<in> set fs" "t \<in> set (trees f)"
-  shows "derives cfg [\<SS> cfg] inp"
+  assumes "wf_\<G> \<G>" "is_word \<G> \<omega>" "nonempty_derives \<G>"
+  assumes "build_trees \<G> \<omega> (Earley\<^sub>L \<G> \<omega>) = Some fs" "f \<in> set fs" "t \<in> set (trees f)"
+  shows "derives \<G> [\<SS> \<G>] \<omega>"
 proof -
-  let ?k = "length (Earley\<^sub>L cfg inp) - 1"
-  define finished where finished_def: "finished = filter_with_index (is_finished cfg inp) (items ((Earley\<^sub>L cfg inp)!?k))"
-  have #: "Some fs = map_option concat (those (map (\<lambda>(_, i). build_trees' (Earley\<^sub>L cfg inp) inp ?k i {i}) finished))"
+  let ?k = "length (Earley\<^sub>L \<G> \<omega>) - 1"
+  define finished where finished_def: "finished = filter_with_index (is_finished \<G> \<omega>) (items ((Earley\<^sub>L \<G> \<omega>)!?k))"
+  have #: "Some fs = map_option concat (those (map (\<lambda>(_, i). build_trees' (Earley\<^sub>L \<G> \<omega>) \<omega> ?k i {i}) finished))"
     using assms(4) build_trees_def finished_def by (metis (full_types))
-  then obtain fss fs' where fss: "Some fss = those (map (\<lambda>(_, i). build_trees' (Earley\<^sub>L cfg inp) inp ?k i {i}) finished)"
+  then obtain fss fs' where fss: "Some fss = those (map (\<lambda>(_, i). build_trees' (Earley\<^sub>L \<G> \<omega>) \<omega> ?k i {i}) finished)"
     "fs' \<in> set fss" "f \<in> set fs'"
     using map_option_concat_those_map_exists assms(5) by fastforce
-  then obtain x i where *: "(x,i) \<in> set finished" "Some fs' =  build_trees' (Earley\<^sub>L cfg inp) inp ?k i {i}"
+  then obtain x i where *: "(x,i) \<in> set finished" "Some fs' =  build_trees' (Earley\<^sub>L \<G> \<omega>) \<omega> ?k i {i}"
     using those_map_exists[OF fss(1,2)] by auto
-  have k: "?k < length (Earley\<^sub>L cfg inp)" "?k \<le> length inp"
+  have k: "?k < length (Earley\<^sub>L \<G> \<omega>)" "?k \<le> length \<omega>"
     by (simp_all add: Earley\<^sub>L_def assms(1))
-  have i: "i < length ((Earley\<^sub>L cfg inp) ! ?k)"
+  have i: "i < length ((Earley\<^sub>L \<G> \<omega>) ! ?k)"
     using index_filter_with_index_lt_length * items_def finished_def by (metis length_map)
-  have x: "x = item ((Earley\<^sub>L cfg inp)!?k!i)"
+  have x: "x = item ((Earley\<^sub>L \<G> \<omega>)!?k!i)"
     using * i filter_with_index_nth items_def nth_map finished_def by metis
-  have finished: "is_finished cfg inp x"
+  have finished: "is_finished \<G> \<omega> x"
     using * filter_with_index_P finished_def by metis
-  moreover have "x \<in> set (items ((Earley\<^sub>L cfg inp) ! ?k))"
+  moreover have "x \<in> set (items ((Earley\<^sub>L \<G> \<omega>) ! ?k))"
     using x by (auto simp: items_def; metis One_nat_def i imageI nth_mem)
-  ultimately have "(\<exists>x \<in> set (items ((Earley\<^sub>L cfg inp) ! length inp)). is_finished cfg inp x)"
-    by (metis assms(1) is_finished_def k(1) wf_bins_Earley\<^sub>L wf_bins_kth_bin)    
-  hence "earley_recognized_it (Earley\<^sub>L cfg inp) cfg inp"
-    using earley_recognized_it_def by blast
+  ultimately have "recognizing (bins (Earley\<^sub>L \<G> \<omega>)) \<G> \<omega>"
+    by (meson k(1) kth_bin_sub_bins recognizing_def subsetD)
   thus ?thesis
-    using correctness_list assms by blast
+    using correctness_Earley\<^sub>L assms by blast
 qed
 
 theorem termination_build_tree_Earley\<^sub>L:
-  assumes "wf_\<G> cfg" "nonempty_derives cfg" "derives cfg [\<SS> cfg] inp"
-  shows "\<exists>fs. build_trees cfg inp (Earley\<^sub>L cfg inp) = Some fs"
+  assumes "wf_\<G> \<G>" "nonempty_derives \<G>" "derives \<G> [\<SS> \<G>] \<omega>"
+  shows "\<exists>fs. build_trees \<G> \<omega> (Earley\<^sub>L \<G> \<omega>) = Some fs"
 proof -
-  let ?k = "length (Earley\<^sub>L cfg inp) - 1"
-  define finished where finished_def: "finished = filter_with_index (is_finished cfg inp) (items ((Earley\<^sub>L cfg inp)!?k))"
-  have "\<forall>f \<in> set finished. (Earley\<^sub>L cfg inp, inp, ?k, snd f, {snd f}) \<in> wf_trees_input"
+  let ?k = "length (Earley\<^sub>L \<G> \<omega>) - 1"
+  define finished where finished_def: "finished = filter_with_index (is_finished \<G> \<omega>) (items ((Earley\<^sub>L \<G> \<omega>)!?k))"
+  have "\<forall>f \<in> set finished. (Earley\<^sub>L \<G> \<omega>, \<omega>, ?k, snd f, {snd f}) \<in> wf_trees_input"
   proof standard
     fix f
     assume a: "f \<in> set finished"
     then obtain x i where *: "(x,i) = f"
       by (metis surj_pair)
-    have "sound_ptrs inp (Earley\<^sub>L cfg inp)"
+    have "sound_ptrs \<omega> (Earley\<^sub>L \<G> \<omega>)"
       using sound_mono_ptrs_Earley\<^sub>L assms by blast
-    moreover have "?k < length (Earley\<^sub>L cfg inp)"
+    moreover have "?k < length (Earley\<^sub>L \<G> \<omega>)"
       by (simp add: Earley\<^sub>L_def assms(1))
-    moreover have "i < length ((Earley\<^sub>L cfg inp)!?k)"
+    moreover have "i < length ((Earley\<^sub>L \<G> \<omega>)!?k)"
       using index_filter_with_index_lt_length a * items_def finished_def by (metis length_map)
-    ultimately show "(Earley\<^sub>L cfg inp, inp, ?k, snd f, {snd f}) \<in> wf_trees_input"
+    ultimately show "(Earley\<^sub>L \<G> \<omega>, \<omega>, ?k, snd f, {snd f}) \<in> wf_trees_input"
       using * unfolding wf_trees_input_def by auto
   qed
-  hence "\<forall>fso \<in> set (map (\<lambda>(_, i). build_trees' (Earley\<^sub>L cfg inp) inp ?k i {i}) finished). \<exists>fs. fso = Some fs"
+  hence "\<forall>fso \<in> set (map (\<lambda>(_, i). build_trees' (Earley\<^sub>L \<G> \<omega>) \<omega> ?k i {i}) finished). \<exists>fs. fso = Some fs"
     using build_trees'_termination by fastforce
-  then obtain fss where fss: "Some fss = those (map (\<lambda>(_, i). build_trees' (Earley\<^sub>L cfg inp) inp ?k i {i}) finished)"
+  then obtain fss where fss: "Some fss = those (map (\<lambda>(_, i). build_trees' (Earley\<^sub>L \<G> \<omega>) \<omega> ?k i {i}) finished)"
     by (smt (verit, best) those_Some)
-  then obtain fs where fs: "Some fs = map_option concat (those (map (\<lambda>(_, i). build_trees' (Earley\<^sub>L cfg inp) inp ?k i {i}) finished))"
+  then obtain fs where fs: "Some fs = map_option concat (those (map (\<lambda>(_, i). build_trees' (Earley\<^sub>L \<G> \<omega>) \<omega> ?k i {i}) finished))"
     by (metis map_option_eq_Some)
   show ?thesis
     using finished_def fss fs build_trees_def by (metis (full_types))
